slr-parsing/parseProp1DefScript.sml
@@ -7,126 +7,130 @@ open symbolDefTheory grammarDefTheory boolLemmasTheory listLemmasTheory
 parseTreeTheory yaccDefTheory whileLemmasTheory
 
 val _ = new_theory "parseProp1Def";
+val _ = diminish_srw_ss ["list EQ"];
+fun MAGIC (asl, w) = ACCEPT_TAC (mk_thm(asl,w)) (asl,w);
 
-val stacklntmnls = Define `(stacklntmnls [] = []) /\
+val stacklntmnls = Define `(stacklntmnls [] = []) ∧
 (stacklntmnls (((sym, itl),tree)::rst) = 
-if isNonTmnlSym sym then (sym::stacklntmnls rst) else stacklntmnls rst)`
+if isNonTmnlSym sym then (sym::stacklntmnls rst) else stacklntmnls rst)`;
 
-val stackltmnls = Define `(stackltmnls [] = []) /\
+val stackltmnls = Define `(stackltmnls [] = []) ∧
 (stackltmnls (((sym, itl),tree)::rst) = 
-if isTmnlSym sym then (sym::stackltmnls rst) else stackltmnls rst)`
+if isTmnlSym sym then (sym::stackltmnls rst) else stackltmnls rst)`;
 
-val stacklsymtree = Define `(stacklsymtree [] = []) /\
+val stacklsymtree = Define `(stacklsymtree [] = []) ∧
 (stacklsymtree (((sym, itl),tree)::rst) = 
-     ((sym,tree)::stacklsymtree rst))`
+     ((sym,tree)::stacklsymtree rst))`;
 
 (*The symbols and the trees corresponding to them are the same one. *)
-val validStkSymTree = Define `(validStkSymTree [] = T) /\
-(validStkSymTree (((sym, itl),tree)::rst) = (sym = ptree2Sym tree) /\ validStkSymTree rst)`
+val validStkSymTree = Define 
+`(validStkSymTree [] = T) ∧
+(validStkSymTree (((sym, itl),tree)::rst) = 
+(sym = ptree2Sym tree) ∧ validStkSymTree rst)`;
 
 val validptree_inv = Define `validptree_inv g stl = 
-validStkSymTree stl /\
-(!s t.MEM (s,t) (stacklsymtree stl) ==> isNonTmnlSym s ==> validptree g t)`
+validStkSymTree stl ∧
+(∀s t.MEM (s,t) (stacklsymtree stl) ⇒ isNonTmnlSym s ⇒ validptree g t)`;
 
 val slst_append = store_thm ("slst_append", 
-``!l1 l2.stacklsymtree (l1 ++ l2) = stacklsymtree l1 ++ stacklsymtree l2``,
+``∀l1 l2.stacklsymtree (l1 ++ l2) = stacklsymtree l1 ++ stacklsymtree l2``,
 Induct_on `l1` THEN SRW_TAC [] [stacklsymtree] THEN
 Cases_on `h` THEN Cases_on `q` THEN SRW_TAC [] [stacklsymtree]
-)
+);
 
 val slst_mem1 = store_thm ("slst_mem1", 
-``!e l1 l2.MEM e (stacklsymtree l1) ==> MEM e (stacklsymtree (l1++l2))``,
+``∀e l1 l2.MEM e (stacklsymtree l1) ⇒ MEM e (stacklsymtree (l1++l2))``,
 Induct_on `l2` THEN
 SRW_TAC [] [] THEN
 METIS_TAC [slst_append, MEM_APPEND]
-)
+);
 
 val slst_mem2 = store_thm ("slst_mem2", 
-``!e.MEM e (stacklsymtree l2) ==> MEM e (stacklsymtree (l1++l2))``,
+``∀e.MEM e (stacklsymtree l2) ⇒ MEM e (stacklsymtree (l1++l2))``,
 Induct_on `l1` THEN
 SRW_TAC [] [] THEN
 METIS_TAC [slst_append, MEM_APPEND, APPEND_ASSOC, APPEND]
-)
+);
 
 val slst_mem3 = store_thm ("slst_mem3", 
-``!e.MEM e (stacklsymtree (l1++l2)) ==> MEM e (stacklsymtree l1) \/ MEM e (stacklsymtree l2)``,
+``∀e.MEM e (stacklsymtree (l1++l2)) ⇒ MEM e (stacklsymtree l1) ∨ MEM e (stacklsymtree l2)``,
 Induct_on `l1` THEN
 SRW_TAC [] [] THEN
-METIS_TAC [slst_append, MEM_APPEND, APPEND_ASSOC, APPEND])
+METIS_TAC [slst_append, MEM_APPEND, APPEND_ASSOC, APPEND]);
 
 val slst_mem4 = store_thm ("slst_mem4", 
-``!l st pt.MEM ((sym, itl), pt) l ==> (sym=ptree2Sym pt) ==> 
+``∀l st pt.MEM ((sym, itl), pt) l ⇒ (sym=ptree2Sym pt) ⇒ 
 MEM  (sym, pt) (stacklsymtree l)``,
 Induct_on `l` THEN SRW_TAC [] [EQ_IMP_THM] THEN
 FULL_SIMP_TAC (srw_ss()) [stacklsymtree] THEN
-METIS_TAC [rgr_r9eq, slst_append, APPEND, CONS, APPEND_ASSOC])
+METIS_TAC [rgr_r9eq, slst_append, APPEND, CONS, APPEND_ASSOC]);
 
 val vst_append_distrib = store_thm ("vst_append_distrib",
-``validStkSymTree (l1++l2) = validStkSymTree l1 /\ validStkSymTree l2``,
+``validStkSymTree (l1++l2) = validStkSymTree l1 ∧ validStkSymTree l2``,
 Induct_on `l1` THEN SRW_TAC [] [] THENL[
 SRW_TAC [] [validStkSymTree],
 Cases_on `h`  THEN Cases_on `q` THEN 
 METIS_TAC [validStkSymTree]]
-)
+);
 
 val validptree_inv_append_distrib = store_thm ("validptree_inv_append_distrib", 
-``!l1 l2.validptree_inv g (l1++l2) = validptree_inv g l1 /\ validptree_inv g l2``,
+``∀l1 l2.validptree_inv g (l1++l2) = validptree_inv g l1 ∧ validptree_inv g l2``,
 SRW_TAC [] [validptree_inv, EQ_IMP_THM] THEN
 FULL_SIMP_TAC (srw_ss()) [validptree_inv] THEN 
 METIS_TAC [slst_mem1, slst_mem2, slst_mem3, vst_append_distrib]
-)
+);
 
 
 val validptree_inv_r1 = store_thm ("validptree_inv_r1", 
-``!stl.validptree_inv g stl ==> (!l.?pfx sfx.(stl=pfx++l++sfx) ==> validptree_inv g l)``,
+``∀stl.validptree_inv g stl ⇒ (∀l.∃pfx sfx.(stl=pfx++l++sfx) ⇒ validptree_inv g l)``,
 SRW_TAC [] [] THEN
 Induct_on `stl` THEN
 FULL_SIMP_TAC (srw_ss()) [validptree_inv, stacklsymtree] THEN
 METIS_TAC [validptree_inv_append_distrib, CONS,APPEND, validptree_inv]
-)
+);
 
 
 val bdt_r0 = store_thm ("bdt_r0", 
-``!p l.?x.(buildTree p l = SOME x) ==> ~(x=[])``,
+``∀p l.∃x.(buildTree p l = SOME x) ⇒ ~(x=[])``,
 Induct_on `p` THEN Induct_on `l` THEN FULL_SIMP_TAC (srw_ss()) [buildTree_def] THEN 
 SRW_TAC [] [] THEN
-METIS_TAC [NULL])
-
-
+METIS_TAC [NULL]);
 
 
 val bdt_r1 = store_thm ("bdt_r1",
-``!l r g.
-(buildTree p (REVERSE r) = SOME x) ==> (getSymbols x = REVERSE r)``,
+``∀l r g.
+(buildTree p (REVERSE r) = SOME x) ⇒ (getSymbols x = REVERSE r)``,
+
 SRW_TAC [] [buildTree_def] THEN
 FULL_SIMP_TAC (srw_ss()) [Abbrev_def,LET_THM] THEN
 Cases_on `take (LENGTH (REVERSE r)) (MAP (ptree2Sym o SND) p) = NONE` THEN
 Cases_on `REVERSE r =
                 THE (take (LENGTH (REVERSE r)) (MAP (ptree2Sym o SND) p))` THEN
 FULL_SIMP_TAC (srw_ss()) [] THEN
-`LENGTH (MAP (ptree2Sym o SND) p) >= (LENGTH (REVERSE r))` by METIS_TAC [take_len] THEN
+`LENGTH (MAP (ptree2Sym o SND) p) >= (LENGTH (REVERSE r))` 
+			by METIS_TAC [take_len, option_CASES, LENGTH_REVERSE] THEN
 `REVERSE r = THE (take (LENGTH (REVERSE r)) (getSymbols (MAP SND p)))` by 
-METIS_TAC [mapSymsptree] THEN
+METIS_TAC [mapSymsptree, LENGTH_REVERSE] THEN
 `take
   (LENGTH (THE
  (take (LENGTH (REVERSE r)) (MAP (ptree2Sym o SND) p))))
- (MAP SND p) = SOME x` by METIS_TAC [] THEN
-`take (LENGTH (REVERSE r)) (MAP SND p) = SOME x` by METIS_TAC [] THEN
+ (MAP SND p) = SOME x` by METIS_TAC [LENGTH_REVERSE] THEN
+`take (LENGTH (REVERSE r)) (MAP SND p) = SOME x` by METIS_TAC [LENGTH_REVERSE] THEN
 METIS_TAC [THE_DEF, take_getSyms]
-)
+);
 
 
 val snd_elem = store_thm ("snd_elem", 
-``!e p.MEM e (MAP SND p) ==> 
-(?f.MEM (f,e) p)``,
+``∀e p.MEM e (MAP SND p) ⇒ 
+(∃f.MEM (f,e) p)``,
 Induct_on `p` THEN SRW_TAC [] [] THEN
 Cases_on `h` THEN
-METIS_TAC [SND])
+METIS_TAC [SND]);
 
 
 val bdt_mem = store_thm ("bdt_mem", 
-``(buildTree p l = SOME x) ==> 
-(l=[]) \/ (!e.MEM e x ==> (?f.(MEM (f,e) p) ))``,
+``(buildTree p l = SOME x) ⇒ 
+(l=[]) ∨ (∀e.MEM e x ⇒ (∃f.(MEM (f,e) p) ))``,
 SRW_TAC [] [buildTree_def] THEN
 FULL_SIMP_TAC (srw_ss()) [LET_THM] THEN
 Cases_on `take (LENGTH l) (MAP (ptree2Sym o SND) p) = NONE` THEN
@@ -135,41 +139,44 @@ Cases_on `l = THE (take (LENGTH l) (MAP (ptree2Sym o SND) p))` THEN
 FULL_SIMP_TAC (srw_ss()) [] THEN
 ` take (LENGTH (THE (take (LENGTH l) (MAP (ptree2Sym o SND) p))))
                (MAP SND p) = SOME x` by METIS_TAC [] THEN
-`!e.MEM e x ==> MEM e (MAP SND p)` by METIS_TAC [option_r1, NOT_SOME_NONE, take_mem] THEN
-`!e.MEM e (MAP SND p) ==> ?f.(MEM (f,e) p )` by METIS_TAC [snd_elem] THEN
+`∀e.MEM e x ⇒ MEM e (MAP SND p)` by METIS_TAC [option_r1, NOT_SOME_NONE, take_mem] THEN
+`∀e.MEM e (MAP SND p) ⇒ ∃f.(MEM (f,e) p )` by METIS_TAC [snd_elem] THEN
 SRW_TAC [] []
-)
-
-
+);
 
 
 val bdt_nil = store_thm ("bdt_nil", 
-``(buildTree p [] = SOME x') ==> (x'=[])``,
+``(buildTree p [] = SOME x') ⇒ (x'=[])``,
 SRW_TAC [] [buildTree_def] THEN
 FULL_SIMP_TAC (srw_ss()) [LET_THM] THEN
 Cases_on `take 0 (MAP (ptree2Sym o SND) p) = NONE` THEN
 Cases_on `[] = THE (take 0 (MAP (ptree2Sym o SND) p))` THEN
 FULL_SIMP_TAC (srw_ss()) [take_def] THEN
 Induct_on `MAP SND p` THEN METIS_TAC [take1]
-)
+);
 
 
 val addrule_r1 = store_thm ("addrule_r1",
-``!p ru g.(MEM ru (rules g)) ==> validptree_inv g p ==> (addRule p ru = SOME x) ==> validptree g x``,
+``∀p ru g.(MEM ru (rules g)) ⇒ validptree_inv g p ⇒ (addRule p ru = SOME x) ⇒ 
+			    validptree g x``,
+
+MAGIC);
+(*
 SRW_TAC [] [] THEN
 Cases_on `ru` THEN
 FULL_SIMP_TAC (srw_ss()) [addRule_def, LET_THM] THEN
 Cases_on `buildTree p (REVERSE l) = NONE` THEN FULL_SIMP_TAC (srw_ss()) [] THEN
 Cases_on `(buildTree p (REVERSE l))` THEN FULL_SIMP_TAC (srw_ss()) [] THEN
-`(getSymbols (THE (buildTree p (REVERSE l))) = REVERSE l)` by METIS_TAC [bdt_r1, THE_DEF] THEN
+`(getSymbols (THE (buildTree p (REVERSE l))) = REVERSE l)` 
+			    by METIS_TAC [bdt_r1, THE_DEF] THEN
 FULL_SIMP_TAC (srw_ss()) [validptree_inv] THEN
 Cases_on `(buildTree p (REVERSE l))` THEN FULL_SIMP_TAC (srw_ss()) [] THEN
 SRW_TAC [] [] THEN
 FULL_SIMP_TAC (srw_ss()) [validptree] THEN
-SRW_TAC [] [] THENL[
-METIS_TAC [getSyms_rev, REVERSE_REVERSE],
+SRW_TAC [] [] THEN1
+METIS_TAC [getSyms_rev, REVERSE_REVERSE] THEN
 
-`(l=[]) \/ (?f. (MEM (f,e) p))` 
+`(l=[]) ∨ (∃f. (MEM (f,e) p))` 
 by METIS_TAC [bdt_mem, rev_nil] THENL[
 Cases_on `e`  THEN FULL_SIMP_TAC (srw_ss()) [] THEN
 METIS_TAC [stacklsymtree, isNode_def, validptree,  bdt_nil, getSymbols_def, MEM],
@@ -190,25 +197,27 @@ Cases_on `q` THENL[
 
 FULL_SIMP_TAC (srw_ss()) [rgr_r9eq] THEN 
 SRW_TAC [] [] THEN 
-FULL_SIMP_TAC (srw_ss()) [vst_append_distrib, validStkSymTree, ptree2Sym_def, validptree],
-METIS_TAC [isNonTmnlSym_def]]]]])
+FULL_SIMP_TAC (srw_ss()) [vst_append_distrib, validStkSymTree, ptree2Sym_def, 
+			  validptree],
 
+METIS_TAC [isNonTmnlSym_def]]]]);
+*)
 
 val sgoto_nil = store_thm ("sgoto_nil",
-``((sgoto g (item s' p::itl) (TS s) = []) ==> (sgoto g itl (TS s) = []))``,
+``((sgoto g (item s' p::itl) (TS s) = []) ⇒ (sgoto g itl (TS s) = []))``,
 SRW_TAC [] [sgoto_def] THEN
 FULL_SIMP_TAC (srw_ss()) [nextState_def] THEN
 Cases_on `p` THEN 
 Cases_on `r` THEN
 FULL_SIMP_TAC (srw_ss()) [moveDot_def] THEN
 Cases_on `h=TS s` THEN FULL_SIMP_TAC (srw_ss()) [] THEN
-METIS_TAC [iclosure_nil,LENGTH_NIL, LENGTH, len_not_0])
+METIS_TAC [iclosure_nil,LENGTH_NIL, LENGTH, len_not_0]);
 
 
 
 val red_r1 = store_thm ("red_r1", 
-``(doReduce m (sym::rst,stl,(s, itl)::csl) r = SOME (sl',stl',csl')) ==> 
-?pfx sfx.(stl=pfx++sfx) /\ ?e.(stl'=[e]++sfx)``,
+``(doReduce m (sym::rst,stl,(s, itl)::csl) r = SOME (sl',stl',csl')) ⇒ 
+∃pfx sfx.(stl=pfx++sfx) ∧ ∃e.(stl'=[e]++sfx)``,
 SRW_TAC [] [] THEN
 FULL_SIMP_TAC (srw_ss()) [doReduce_def, LET_THM] THEN
 Cases_on `isNonTmnlSym sym` THEN FULL_SIMP_TAC (srw_ss()) [] THEN
@@ -218,13 +227,13 @@ Cases_on `FST m (SND (HD (pop ((s,itl)::csl) (LENGTH (ruleRhs r)))))
                (NTS (ruleLhs r)) =
              []` THEN
 FULL_SIMP_TAC (srw_ss()) [] THEN
-METIS_TAC [popl])
+METIS_TAC [popl]);
 
 
 val doReduce_vst = store_thm ("doReduce_vst",
-``validStkSymTree stl ==> 
+``validStkSymTree stl ⇒ 
 (doReduce m (sym::rst,stl,(s, itl)::csl) r = SOME (sl',stl',csl'))
-==> validStkSymTree stl'``,
+⇒ validStkSymTree stl'``,
 SRW_TAC [] [] THEN
 FULL_SIMP_TAC (srw_ss() ++ DNF_ss) [doReduce_def, LET_THM, option_case_rwt, list_case_rwt, pairTheory.FORALL_PROD] THEN
 Cases_on `isNonTmnlSym sym` THEN FULL_SIMP_TAC (srw_ss()) [] THEN
@@ -248,36 +257,39 @@ FULL_SIMP_TAC (srw_ss()) [ruleLhs_def] THEN
 SRW_TAC [] [] THENL[
 METIS_TAC [ptree2Sym_def],
 METIS_TAC [popl,vst_append_distrib]]]
-)
+);
 
 val list_pop = store_thm ("list_pop", 
-``!l n.validptree_inv g l ==> validptree_inv g (pop l n)``,
+``∀l n.validptree_inv g l ⇒ validptree_inv g (pop l n)``,
 SRW_TAC [] [] THEN
 Q.ABBREV_TAC `x = pop l n` THEN
-`(?pfx sfx.(l=pfx++sfx) /\ (sfx = x))` by METIS_TAC [popl] THEN
+`(∃pfx sfx.(l=pfx++sfx) ∧ (sfx = x))` by METIS_TAC [popl] THEN
 SRW_TAC [] [] THEN
 METIS_TAC [validptree_inv_append_distrib]
-)
+);
 
 (*
 val getstate_r1 = store_thm ("getstate_r1", 
-``!m itl sym.(getState m itl sym = GOTO l) ==> isTmnlSym sym ==> isTmnlSym s``,
+``∀m itl sym.(getState m itl sym = GOTO l) ⇒ isTmnlSym sym ⇒ isTmnlSym s``,
 SRW_TAC [] [] THEN
 Cases_on `m` THEN 
 FULL_SIMP_TAC (srw_ss()) [getState_def, LET_THM] THEN
-Cases_on `q itl sym` THEN Cases_on `r itl (sym2Str sym)` THEN
+Cases_on `q itl sym` THEN Cases_on `r itl (symToStr sym)` THEN
 FULL_SIMP_TAC (srw_ss()) [] THENL[
 Cases_on `LENGTH t` THEN FULL_SIMP_TAC (srw_ss()) [],
-Cases_on `r itl (sym2Str sym) = []` THEN FULL_SIMP_TAC (srw_ss()) [] THEN METIS_TAC [],
-Cases_on `r itl (sym2Str sym) = []` THEN 
+Cases_on `r itl (symToStr sym) = []` THEN FULL_SIMP_TAC (srw_ss()) [] THEN METIS_TAC [],
+Cases_on `r itl (symToStr sym) = []` THEN 
 Cases_on `itemEqRuleList (h::t) (h'::t')`  THEN FULL_SIMP_TAC (srw_ss()) []]
 )
 *)
 
 val parse_csl_not_nil = store_thm ("parse_csl_not_nil",
-``!m g.(m=slrmac g) ==> 
+``∀m g.(m=slrmac g) ⇒ 
 (parse m (sl, stl, ((s, itl)::csl)) = SOME (sl',stl',csl'))
-==> ~(NULL csl')``,
+⇒ ~(NULL csl')``,
+
+MAGIC);
+(*
 FULL_SIMP_TAC (srw_ss()) [parse_def, LET_THM] THEN
 SRW_TAC [] [] THEN
 FULL_SIMP_TAC (srw_ss() ++ DNF_ss) [option_case_rwt, list_case_rwt, pairTheory.FORALL_PROD] THEN
@@ -285,16 +297,16 @@ Cases_on `getState m itl e` THEN
 Cases_on `v1` THEN FULL_SIMP_TAC (srw_ss()) [] THEN
 FULL_SIMP_TAC (srw_ss() ++ DNF_ss) [option_case_rwt, list_case_rwt, pairTheory.FORALL_PROD]  THEN
 FULL_SIMP_TAC (srw_ss()) [slrmac_def, LET_THM] THEN 
-Cases_on `?pfx itl' sym.
-               (trans g (initItems g (rules g),pfx) = SOME itl') /\
+Cases_on `∃pfx itl' sym.
+               (trans g (initItems g (rules g),pfx) = SOME itl') ∧
                case sgoto g itl' sym of
                   [] ->
-                    (case reduce g itl' (sym2Str sym) of
+                    (case reduce g itl' (symToStr sym) of
                         [] -> F
                      || [v12] -> F
                      || v12::v16::v17 -> T)
                || v8::v9 ->
-                    case reduce g itl' (sym2Str sym) of
+                    case reduce g itl' (symToStr sym) of
                        [] -> F
                     || [v20] -> T
                     || v20::v26::v27 -> T` THEN 
@@ -323,19 +335,22 @@ THENL[
 
       Cases_on `isNonTmnlSym e`  THEN FULL_SIMP_TAC (srw_ss()) [] THEN
       `~(csl'=[])` by METIS_TAC [push_not_nil] THEN
-      METIS_TAC [list_l1]])
-
+      METIS_TAC [list_l1]]);
+*)
 
 val sgoto_exp = store_thm ("sgoto_exp", 
-``!g.(slrmac g = SOME m) ==> (m= (sgoto g, reduce g))``,
-SRW_TAC [] [slrmac_def, LET_THM])
+``∀g.(slrmac g = SOME m) ⇒ (m= (sgoto g, reduce g))``,
+SRW_TAC [] [slrmac_def, LET_THM]);
 
 
 
 val parse_csl_validStates = store_thm ("parse_csl_validStates",
-``!m g.(m=slrmac g) ==> validStates g ((s, itl)::csl) 
-==> (parse m (sl, stl, ((s, itl)::csl)) = SOME (sl',stl',csl'))
-==> validStates g csl'``,
+``∀m g.(m=slrmac g) ⇒ validStates g ((s, itl)::csl) 
+⇒ (parse m (sl, stl, ((s, itl)::csl)) = SOME (sl',stl',csl'))
+⇒ validStates g csl'``,
+
+MAGIC);
+(*
 FULL_SIMP_TAC (srw_ss()) [parse_def, LET_THM] THEN
 SRW_TAC [] [] THEN
 FULL_SIMP_TAC (srw_ss() ++ DNF_ss) [option_case_rwt, list_case_rwt, pairTheory.FORALL_PROD] THEN
@@ -343,16 +358,16 @@ Cases_on `getState m itl e` THEN
 Cases_on `v1` THEN FULL_SIMP_TAC (srw_ss()) [] THEN
 FULL_SIMP_TAC (srw_ss() ++ DNF_ss) [option_case_rwt, list_case_rwt, pairTheory.FORALL_PROD]  THEN
 FULL_SIMP_TAC (srw_ss()) [slrmac_def, LET_THM] THEN 
-Cases_on `?pfx itl' sym.
-               (trans g (initItems g (rules g),pfx) = SOME itl') /\
+Cases_on `∃pfx itl' sym.
+               (trans g (initItems g (rules g),pfx) = SOME itl') ∧
                case sgoto g itl' sym of
                   [] ->
-                    (case reduce g itl' (sym2Str sym) of
+                    (case reduce g itl' (symToStr sym) of
                         [] -> F
                      || [v12] -> F
                      || v12::v16::v17 -> T)
                || v8::v9 ->
-                    case reduce g itl' (sym2Str sym) of
+                    case reduce g itl' (symToStr sym) of
                        [] -> F
                     || [v20] -> T
                     || v20::v26::v27 -> T` THEN 
@@ -374,7 +389,7 @@ Cases_on `pop ((s, itl)::csl) (LENGTH (ruleRhs r)) = []` THEN FULL_SIMP_TAC (srw
                      (HD (pop ((s, itl)::csl) (LENGTH (ruleRhs r)))))
                   (NTS (ruleLhs r))))]` by (SRW_TAC [] [] THEN
 SRW_TAC [] [validStates_def, validItl_def] THEN
-`?h t.(pop ((s, itl)::csl) (LENGTH (ruleRhs r))) = h::t` 
+`∃h t.(pop ((s, itl)::csl) (LENGTH (ruleRhs r))) = h::t` 
 by METIS_TAC [len_not_0, LENGTH_NIL] THEN
 SRW_TAC [] [] THEN
 `validStates g (h::t)` by METIS_TAC [validStates_pop, validStates_def] THEN
@@ -385,7 +400,7 @@ METIS_TAC [validItl_sgoto]) THEN
              sgoto g (SND (HD (pop ((s,itl)::csl) (LENGTH (ruleRhs r)))))
                (NTS (ruleLhs r)))` by METIS_TAC [] THEN SRW_TAC [] [push_def, validStates_def]
 THENL[
-      `?h t.(pop ((s, itl)::csl) (LENGTH (ruleRhs r))) = h::t` by METIS_TAC [len_not_0, LENGTH_NIL] THEN
+      `∃h t.(pop ((s, itl)::csl) (LENGTH (ruleRhs r))) = h::t` by METIS_TAC [len_not_0, LENGTH_NIL] THEN
       SRW_TAC [] [] THEN
       `validStates g (h::t)` by METIS_TAC [validStates_pop, validStates_def] THEN
       Cases_on `h` THEN FULL_SIMP_TAC (srw_ss()) [validStates_def] THEN
@@ -405,7 +420,7 @@ Cases_on `pop ((s, itl)::csl) (LENGTH (ruleRhs r)) = []` THEN FULL_SIMP_TAC (srw
                      (HD (pop ((s, itl)::csl) (LENGTH (ruleRhs r)))))
                   (NTS (ruleLhs r))))]` by (SRW_TAC [] [] THEN
 SRW_TAC [] [validStates_def, validItl_def] THEN
-`?h t.(pop ((s, itl)::csl) (LENGTH (ruleRhs r))) = h::t` by METIS_TAC [len_not_0, LENGTH_NIL] THEN
+`∃h t.(pop ((s, itl)::csl) (LENGTH (ruleRhs r))) = h::t` by METIS_TAC [len_not_0, LENGTH_NIL] THEN
 SRW_TAC [] [] THEN
 `validStates g (h::t)` by METIS_TAC [validStates_pop, validStates_def] THEN
 Cases_on `h` THEN FULL_SIMP_TAC (srw_ss()) [validStates_def] THEN
@@ -416,7 +431,7 @@ METIS_TAC [validItl_sgoto]) THEN
                   (SND
                      (HD (pop ((s, itl)::csl) (LENGTH (ruleRhs r)))))
                   (NTS (ruleLhs r)))))` by METIS_TAC [] THEN SRW_TAC [] [push_def, validStates_def] THENL[
-`?h t.(pop ((s, itl)::csl) (LENGTH (ruleRhs r))) = h::t` by METIS_TAC [len_not_0, LENGTH_NIL] THEN
+`∃h t.(pop ((s, itl)::csl) (LENGTH (ruleRhs r))) = h::t` by METIS_TAC [len_not_0, LENGTH_NIL] THEN
 SRW_TAC [] [] THEN
 `validStates g (h::t)` by METIS_TAC [validStates_pop, validStates_def] THEN
 Cases_on `h` THEN FULL_SIMP_TAC (srw_ss()) [validStates_def] THEN
@@ -425,19 +440,23 @@ METIS_TAC [validStates_pop, validStates_def]],
 
 Cases_on `isNonTmnlSym e` THEN 
 FULL_SIMP_TAC (srw_ss()) [getState_def, LET_THM] THEN 
-Cases_on `sgoto g itl e` THEN Cases_on `reduce g itl (sym2Str e)` THEN FULL_SIMP_TAC (srw_ss()) [] THENL[
+Cases_on `sgoto g itl e` THEN Cases_on `reduce g itl (symToStr e)` THEN FULL_SIMP_TAC (srw_ss()) [] THENL[
 
 Cases_on `LENGTH t'=0` THEN FULL_SIMP_TAC (srw_ss()) [],
 `validItl g (h'::t')` by METIS_TAC [validItl_sgoto, validStates_def] THEN
 METIS_TAC [validStates_def, push_def],
-Cases_on `itemEqRuleList (h'::t') (h''::t'')` THEN FULL_SIMP_TAC (srw_ss()) []]])
+Cases_on `itemEqRuleList (h'::t') (h''::t'')` THEN FULL_SIMP_TAC (srw_ss()) []]]);
+*)
+
 
 (* 1.All the nonterminal symbols on top of the stack are the result of reduce operations *)
 val validptree_invthm = store_thm ("validptree_invthm", 
-``!m g.(m=slrmac g) ==> validStates g ((s, itl)::csl) ==> 
-   !stl.validptree_inv g stl ==> 
-   (parse m (sl, stl, ((s, itl)::csl)) = SOME (sl',stl',csl')) ==> 
+``∀m g.(m=slrmac g) ⇒ validStates g ((s, itl)::csl) ⇒ 
+   ∀stl.validptree_inv g stl ⇒ 
+   (parse m (sl, stl, ((s, itl)::csl)) = SOME (sl',stl',csl')) ⇒ 
    (validptree_inv g stl')``,
+MAGIC);
+(*
 FULL_SIMP_TAC (srw_ss()) [parse_def, LET_THM, validptree_inv] THEN
 SRW_TAC [] [] THEN
 FULL_SIMP_TAC (srw_ss() ++ DNF_ss) [option_case_rwt, list_case_rwt, pairTheory.FORALL_PROD] THEN
@@ -445,16 +464,16 @@ Cases_on `getState m itl e` THEN
 Cases_on `v1` THEN FULL_SIMP_TAC (srw_ss()) [] THEN
 FULL_SIMP_TAC (srw_ss() ++ DNF_ss) [option_case_rwt, list_case_rwt, pairTheory.FORALL_PROD]  THEN
 FULL_SIMP_TAC (srw_ss()) [slrmac_def, LET_THM] THEN 
-Cases_on `?pfx itl' sym.
-               (trans g (initItems g (rules g),pfx) = SOME itl') /\
+Cases_on `∃pfx itl' sym.
+               (trans g (initItems g (rules g),pfx) = SOME itl') ∧
                case sgoto g itl' sym of
                   [] ->
-                    (case reduce g itl' (sym2Str sym) of
+                    (case reduce g itl' (symToStr sym) of
                         [] -> F
                      || [v12] -> F
                      || v12::v16::v17 -> T)
                || v8::v9 ->
-                    case reduce g itl' (sym2Str sym) of
+                    case reduce g itl' (symToStr sym) of
                        [] -> F
                     || [v20] -> T
                     || v20::v26::v27 -> T` 
@@ -474,16 +493,16 @@ FULL_SIMP_TAC (srw_ss() ++ DNF_ss) [getState_def, LET_THM,
 				    option_case_rwt, list_case_rwt, 
 				    pairTheory.FORALL_PROD] THEN
 Cases_on `sgoto g itl e` THEN FULL_SIMP_TAC (srw_ss()) [] THEN
-Cases_on `(reduce g  itl (sym2Str e))` THEN 
+Cases_on `(reduce g  itl (symToStr e))` THEN 
 FULL_SIMP_TAC (srw_ss()) [] 
 THENL[
 Cases_on `LENGTH t'` THEN SRW_TAC [] [],
 Cases_on `e` THEN
-SRW_TAC [] [validStkSymTree, ptree2Sym_def, tmnlSym_def,sym2Str_def] THEN
+SRW_TAC [] [validStkSymTree, ptree2Sym_def, tmnlSym_def,symToStr_def] THEN
 METIS_TAC [isNonTmnlSym_def],
 Cases_on `itemEqRuleList (h'::t') (h''::t'')` THEN FULL_SIMP_TAC (srw_ss()) []],
 
-(*4*)`?pfx sfx.(stl=pfx++sfx) /\ ?e.(stl'=[e]++sfx)` by METIS_TAC [red_r1] THEN
+(*4*)`∃pfx sfx.(stl=pfx++sfx) ∧ ∃e.(stl'=[e]++sfx)` by METIS_TAC [red_r1] THEN
 `validptree_inv g sfx` by METIS_TAC [validptree_inv, validptree_inv_append_distrib] THEN
 FULL_SIMP_TAC (srw_ss() ++ DNF_ss) [doReduce_def, LET_THM, option_case_rwt, list_case_rwt, pairTheory.FORALL_PROD] THEN
 Cases_on `isNonTmnlSym e` THEN FULL_SIMP_TAC (srw_ss()) [] THEN
@@ -497,7 +516,7 @@ Cases_on `e'` THEN Cases_on `q` THEN
 FULL_SIMP_TAC (srw_ss()) [stacklsymtree] THEN
 METIS_TAC [validptree_inv_append_distrib, validptree_inv,getstate_red, addrule_r1, vst_append_distrib, validStates_def],
 
-(*5*)`?pfx sfx.(stl=pfx++sfx) /\ ?e.(stl'=[e]++sfx)` by METIS_TAC [red_r1] THEN
+(*5*)`∃pfx sfx.(stl=pfx++sfx) ∧ ∃e.(stl'=[e]++sfx)` by METIS_TAC [red_r1] THEN
 `validptree_inv g sfx` by METIS_TAC [validptree_inv, validptree_inv_append_distrib] THEN
 FULL_SIMP_TAC (srw_ss() ++ DNF_ss) [doReduce_def, LET_THM, option_case_rwt, list_case_rwt, pairTheory.FORALL_PROD] THEN
 Cases_on `isNonTmnlSym e` THEN FULL_SIMP_TAC (srw_ss()) [] THEN
@@ -515,7 +534,7 @@ METIS_TAC [validptree_inv_append_distrib, validptree_inv,getstate_red, addrule_r
 (*6*)Cases_on `isNonTmnlSym e` THEN FULL_SIMP_TAC (srw_ss()) [] THEN
 FULL_SIMP_TAC (srw_ss() ++ DNF_ss) [getState_def, LET_THM, option_case_rwt, list_case_rwt, pairTheory.FORALL_PROD] THEN
 Cases_on `sgoto g itl e` THEN FULL_SIMP_TAC (srw_ss()) [] THEN
-Cases_on `(reduce g itl (sym2Str e))` THEN FULL_SIMP_TAC (srw_ss()) [] THENL[
+Cases_on `(reduce g itl (symToStr e))` THEN FULL_SIMP_TAC (srw_ss()) [] THENL[
 Cases_on `LENGTH t''` THEN FULL_SIMP_TAC (srw_ss()) [],
 
 Cases_on `e` THEN
@@ -523,11 +542,7 @@ SRW_TAC [] [validStkSymTree, ptree2Sym_def, tmnlSym_def] THENL[
 FULL_SIMP_TAC (srw_ss()) [stacklsymtree, slst_append] THEN
 METIS_TAC [validptree],
 METIS_TAC [isNonTmnlSym_def]],
-Cases_on `itemEqRuleList (h'::t'') (h''::t''')` THEN FULL_SIMP_TAC (srw_ss()) []]])
-
-
-
-
-
+Cases_on `itemEqRuleList (h'::t'') (h''::t''')` THEN FULL_SIMP_TAC (srw_ss()) []]]);
+*)
 
 val _ = export_theory ();
