slr-parsing/parseProp3DefScript.sml
@@ -4,29 +4,36 @@ open listTheory containerTheory pred_setTheory arithmeticTheory
 relationTheory markerTheory boolSimps optionTheory
 
 open symbolDefTheory grammarDefTheory boolLemmasTheory listLemmasTheory
-parseTreeTheory parserDefTheory yaccDefTheory
+parseTreeTheory yaccDefTheory
 
 val _ = new_theory "parseProp3Def";
+val _ = diminish_srw_ss ["list EQ"];
 
 (* 3. There is an item rule in the current state list that has the
 stack symbols as its pfx and by that it implies that a corresponding
 rule exists in the grammar *)
 
-val stackSymbols = Define `(stackSymbols [] = []) /\
-(stackSymbols (((sym itl), pt)::rst) = sym::stackSymbols rst)`
+val stackSymbols = Define 
+`(stackSymbols [] = []) ∧
+(stackSymbols (((sym itl), pt)::rst) = sym::stackSymbols rst)`;
 
 val prop3  = Define `prop3 g stl = 
-!sym itl pt.MEM ((sym itl), pt) stl ==> isTmnlSym sym ==> ?e.(MEM e itl /\ (?nt sfx.(e=item nt (stackSymbols (TL stl), sfx))))`
+∀sym itl pt.MEM ((sym itl), pt) stl ⇒ isTmnlSym sym 
+    ⇒ ∃e.(MEM e itl ∧ (∃nt sfx.(e=item nt (stackSymbols (TL stl), sfx))))`;
 
 
 val prop3thm = store_thm ("prop3thm", 
-``!m g.(m=slr g) ==> prop3 g stl ==> ((parse m (sl, stl, (state s itl::csl)) = SOME (sl',stl',csl'))) ==> prop3 g stl``,
+``∀m g.(m=slr g) ⇒ prop3 g stl ⇒ 
+((parse m (sl, stl, (state s itl::csl)) = SOME (sl',stl',csl'))) 
+			  ⇒ prop3 g stl``,
+
 FULL_SIMP_TAC (srw_ss()) [parse_def, LET_THM, prop3] THEN
 SRW_TAC [] [] THEN
-FULL_SIMP_TAC (srw_ss() ++ DNF_ss) [option_case_rwt, list_case_rwt, pairTheory.FORALL_PROD] THEN
+FULL_SIMP_TAC (srw_ss() ++ DNF_ss) 
+[option_case_rwt, list_case_rwt, pairTheory.FORALL_PROD] THEN
 Cases_on `getState m itl sym` THEN FULL_SIMP_TAC (srw_ss()) [] THEN
 (* 5 subgoals *)
 METIS_TAC []
-)
+);
 
 val _ = export_theory ();
