slr-parsing/yaccDefScript.sml
@@ -6,46 +6,51 @@ optionTheory rich_listTheory
 
 open symbolDefTheory parseTreeTheory grammarDefTheory listLemmasTheory
 firstSetDefTheory followSetDefTheory containerLemmasTheory
-setLemmasTheory boolLemmasTheory whileLemmasTheory
+setLemmasTheory boolLemmasTheory whileLemmasTheory relationLemmasTheory
 
 val _ = new_theory "yaccDef"
+fun MAGIC (asl, w) = ACCEPT_TAC (mk_thm(asl,w)) (asl,w);
 
 
 val _ = Globals.linewidth := 60
+val _ = diminish_srw_ss ["list EQ"];
 
-val _ = Hol_datatype `item = item of string => symbol list # symbol list`; (*  # symbol list`;*)
+val _ = Hol_datatype 
+`item = item of 'nts => ('nts,'ts) symbol list # ('nts,'ts) symbol list`; 
 
-val _ = type_abbrev ("state", ``:item list``)
+val _ = type_abbrev ("state", ``:('nts,'ts) item list``);
 
-val _ = Hol_datatype `action = REDUCE of rule | GOTO of state | NA`
+val _ = Hol_datatype `action = 
+    REDUCE of ('nts,'ts) rule | GOTO of ('nts,'ts) state | NA`;
 
 
 val getItems = Define `
-(getItems [] s = [])
-/\ (getItems ((rule l r)::rs) s = if (l=s) then (item l ([],r)::getItems rs s) 
-				  else getItems rs s)`
+(getItems [] s = []) ∧ 
+(getItems ((rule l r)::rs) s = if (l=s) then (item l ([],r)::getItems rs s) 
+			       else getItems rs s)`;
 
 (* iclosure :: grammar -> item list -> item list *)
-val iclosure1 = Define `(iclosure1 g [] = []) /\
-(iclosure1 g ((item s (l1,[]))::il) = ((item s (l1,[]))::iclosure1 g il)) /\
+val iclosure1 = Define 
+`(iclosure1 g [] = []) ∧
+(iclosure1 g ((item s (l1,[]))::il) = ((item s (l1,[]))::iclosure1 g il)) ∧
 (iclosure1 g ((item s (l1,TS ts::l2))::il) = 
- (((item s (l1,TS ts::l2)))::iclosure1 g il)) /\
+ (((item s (l1,TS ts::l2)))::iclosure1 g il)) ∧
 (iclosure1 g ((item s (l1,NTS nt::l2))::il) = 
-(getItems (rules g) nt ++ [(item s (l1,NTS nt::l2))] ++ iclosure1 g il))`
+(getItems (rules g) nt ++ [(item s (l1,NTS nt::l2))] ++ iclosure1 g il))`;
 
 
 (* iclosure :: grammar -> item list -> item list *)
-val iclosure1 = Define `(iclosure1 g [] = []) /\
-(iclosure1 g ((item s (l1,[]))::il) = ((item s (l1,[]))::iclosure1 g il)) /\
+val iclosure1 = Define `(iclosure1 g [] = []) ∧
+(iclosure1 g ((item s (l1,[]))::il) = ((item s (l1,[]))::iclosure1 g il)) ∧
 (iclosure1 g ((item s (l1,TS ts::l2))::il) = 
- (((item s (l1,TS ts::l2)))::iclosure1 g il)) /\
+ (((item s (l1,TS ts::l2)))::iclosure1 g il)) ∧
 (iclosure1 g ((item s (l1,NTS nt::l2))::il) = 
-(getItems (rules g) nt ++ [(item s (l1,NTS nt::l2))] ++ iclosure1 g il))`
+(getItems (rules g) nt ++ [(item s (l1,NTS nt::l2))] ++ iclosure1 g il))`;
 
 
 val iclosure_defn = Hol_defn 
 "iclosure_defn" 
-`(iclosure g [] = []) /\
+`(iclosure g [] = []) ∧
 (iclosure g il = 
 	let
 	    ril = rmDupes il
@@ -54,14 +59,23 @@ val iclosure_defn = Hol_defn
 		    al = rmDupes (iclosure1 g ril)
 		in 
 		    if ~(LIST_TO_SET ril = LIST_TO_SET al) then iclosure g al
-		    else al)`
+		    else al)`;
 
 
-val rules2Items = Define `(rules2Items [] = []) /\
-(rules2Items (rule l r::rst) = item l ([], r)::rules2Items rst)`
+val closure = Define
+`closure g itl = 
+      { item sym ([],r) | 
+       ∃l r1 r2 nt sfx. MEM (item l (r1,NTS nt::r2)) itl ∧
+       RTC (derives g) [NTS nt] (NTS sym::sfx) ∧
+       MEM (rule sym r) (rules g) }`;
+
+
+val rules2Items = Define 
+`(rules2Items [] = []) ∧
+(rules2Items (rule l r::rst) = item l ([], r)::rules2Items rst)`;
 
 val iclosure1_mem = store_thm ("iclosure1_mem", 
-``!e l.MEM e l ==> (MEM e (iclosure1 g l))``,
+``∀e l.MEM e l ⇒ (MEM e (iclosure1 g l))``,
 Induct_on `l` THEN SRW_TAC [] [] THENL[
 Cases_on `e`  THEN Cases_on `p` THEN Cases_on `r` THEN SRW_TAC [] [] THENL[
 FULL_SIMP_TAC (srw_ss()) [iclosure1] THEN
@@ -71,32 +85,32 @@ METIS_TAC [rmd_r2_1, MEM, APPEND, CONS, rgr_r9eq, MEM_APPEND]],
 Cases_on `h` THEN Cases_on `p` THEN Cases_on `r` THEN 
 FULL_SIMP_TAC (srw_ss()) [iclosure1] THEN
 Cases_on `h` THEN FULL_SIMP_TAC (srw_ss()) [iclosure1] THEN
-METIS_TAC [rmd_r2_1, MEM, APPEND, CONS, rgr_r9eq, MEM_APPEND]])
+METIS_TAC [rmd_r2_1, MEM, APPEND, CONS, rgr_r9eq, MEM_APPEND]]);
 
 
 
 val iclosure1_not_nil = store_thm ("iclosure1_not_nil", 
-``!g x xs.~(iclosure1 g (x::xs) = [])``,
+``∀g x xs.~(iclosure1 g (x::xs) = [])``,
 Cases_on `x` THEN Cases_on `p` THEN Cases_on `r` THENL[
 SRW_TAC [] [iclosure1, rmDupes_not_nil],
 Cases_on `h` THEN SRW_TAC [] [iclosure1, rmDupes_not_nil] THEN
-Cases_on `getItems (rules g) s'` THEN SRW_TAC [] [iclosure1, rmDupes_not_nil]])
+Cases_on `getItems (rules g) s'` THEN SRW_TAC [] [iclosure1, rmDupes_not_nil]]);
 
 val iclosure1_len = store_thm ("iclosure1_len", 
-``!g l.LENGTH (iclosure1 g l) >= LENGTH (rmDupes l)``,
+``∀g l.LENGTH (iclosure1 g l) >= LENGTH (rmDupes l)``,
 Induct_on `iclosure1 g l` THEN SRW_TAC [] [] THEN
 Induct_on `l` THEN SRW_TAC [] [iclosure1, rmDupes] THENL[
 METIS_TAC [iclosure1_not_nil],
 `~(iclosure1 g (h'::l) = [])` by METIS_TAC [iclosure1_not_nil] THEN
-`!e.MEM e (h'::l) ==> MEM e (iclosure1 g (h'::l))` by METIS_TAC [iclosure1_mem] THEN
+`∀e.MEM e (h'::l) ⇒ MEM e (iclosure1 g (h'::l))` by METIS_TAC [iclosure1_mem] THEN
 `LENGTH (h'::l) >= SUC (LENGTH l)` by FULL_SIMP_TAC (arith_ss) [LENGTH] THEN
 `LENGTH (iclosure1 g (h'::l)) >= LENGTH (rmDupes (h'::l))` 
 by METIS_TAC [mem_subset_len, rmd_r2] THEN
-FULL_SIMP_TAC (arith_ss) [rmDupes, MEM, APPEND, LENGTH]])
+FULL_SIMP_TAC (arith_ss) [rmDupes, MEM, APPEND, LENGTH]]);
 
 val rmd_del_eq_list = 
 store_thm ("rmd_del_eq_list",
- ``!e l.(rmDupes (delete e l) = l) ==>
+ ``∀e l.(rmDupes (delete e l) = l) ⇒
       (rmDupes l = l)``,
 Induct_on `l` THEN SRW_TAC [] [rmDupes,delete_def] 
 THENL[
@@ -107,69 +121,75 @@ THENL[
 	    METIS_TAC [not_mem_delete,MEM,rmd_mem_list],
 
 	    Cases_on `MEM e l` THEN
-	    METIS_TAC [delete_not_mem,MEM,rmd_mem_list,not_mem_delete,delete_mem_list]
+	    METIS_TAC [delete_not_mem,MEM,rmd_mem_list,not_mem_delete,
+		       delete_mem_list]
 	    ]
-      ])
+      ]);
 
 val rules2items_sub = store_thm ("rules2items_sub",
-``!e lhs rs.MEM e (getItems rs lhs) ==> MEM e (rules2Items rs)``,
+``∀e lhs rs.MEM e (getItems rs lhs) ⇒ MEM e (rules2Items rs)``,
 Induct_on `rs` THEN SRW_TAC [] [getItems, rules2Items] THEN
 Cases_on `h` THEN  FULL_SIMP_TAC (srw_ss()) [rules2Items, getItems] THEN
 Cases_on `s=lhs` THEN FULL_SIMP_TAC (srw_ss()) [] THEN
-METIS_TAC [MEM, rules2Items, getItems, APPEND])
+METIS_TAC [MEM, rules2Items, getItems, APPEND]);
 
 val iclosure1_outmem = store_thm ("iclosure1_outmem", 
-``!e l.MEM e (iclosure1 g l) ==> ~(MEM e l) ==> (MEM e (rules2Items (rules g)))``,
+``∀e l.MEM e (iclosure1 g l) ⇒ ~(MEM e l) ⇒ (MEM e (rules2Items (rules g)))``,
 Induct_on `l` THEN SRW_TAC [] [iclosure1] THEN
 Cases_on `h` THEN  Cases_on `p` THEN Cases_on `r` THEN
 FULL_SIMP_TAC (srw_ss()) [iclosure1] THEN
 Cases_on `h` THEN 
 FULL_SIMP_TAC (srw_ss()) [iclosure1] THEN
-METIS_TAC [rmd_r2_2, MEM, MEM_APPEND, rules2items_sub])
+METIS_TAC [rmd_r2_2, MEM, MEM_APPEND, rules2items_sub]);
 
 
 val iclosure1_before_after_len = store_thm ("iclosure1_before_after_len",
-``!l.(CARD (set (iclosure1 g l)) > CARD (set l)) ==> 
+``∀l.(CARD (set (iclosure1 g l)) > CARD (set l)) ⇒ 
 ((CARD (set (rules2Items (rules g)) INTER set (iclosure1 g l)) -
 CARD (set (rules2Items (rules g)) INTER (set l))) > 0)``,
 SRW_TAC [] [] THEN
 `(set l) SUBSET (set (iclosure1 g l))` by METIS_TAC [mem_subset, iclosure1_mem] THEN
-`?e.~(e IN set l) /\ (e IN set (iclosure1  g l))` by METIS_TAC [set_neq, FINITE_LIST_TO_SET] THEN
+`∃e.~(e IN set l) ∧ (e IN set (iclosure1  g l))` by METIS_TAC [set_neq, FINITE_LIST_TO_SET] THEN
 `MEM e (iclosure1 g l)` by METIS_TAC [IN_LIST_TO_SET] THEN
 `~(MEM e l)` by METIS_TAC [IN_LIST_TO_SET] THEN
 `MEM e (rules2Items (rules g))` by METIS_TAC [iclosure1_outmem] THEN
 `e IN set (rules2Items (rules g))` by METIS_TAC [IN_LIST_TO_SET] THEN
 `~(set l= set (iclosure1 g l))` by METIS_TAC [LIST_TO_SET_THM, IN_LIST_TO_SET] THEN
 `(set l) PSUBSET set (iclosure1 g l)` by METIS_TAC [PSUBSET_DEF] THEN
-`CARD (set l) < CARD (set (iclosure1 g l))` by METIS_TAC [CARD_PSUBSET, FINITE_LIST_TO_SET] THEN
-`CARD (set l) < CARD (set (iclosure1 g l))` by METIS_TAC [CARD_PSUBSET, FINITE_LIST_TO_SET] THEN
+`CARD (set l) < CARD (set (iclosure1 g l))` by METIS_TAC [CARD_PSUBSET, 
+							  FINITE_LIST_TO_SET] THEN
+`CARD (set l) < CARD (set (iclosure1 g l))` by METIS_TAC [CARD_PSUBSET, 
+							  FINITE_LIST_TO_SET] THEN
 `CARD (set l INTER (set (rules2Items (rules g)))) 
 < CARD (set (iclosure1 g l) INTER (set (rules2Items (rules g))))` 
 by METIS_TAC [card_same_inter, FINITE_LIST_TO_SET] THEN
-FULL_SIMP_TAC (arith_ss) [INTER_COMM])
+FULL_SIMP_TAC (arith_ss) [INTER_COMM]);
 
 
 val (iclosure, iclosure_ind) = tprove(iclosure_defn,
 WF_REL_TAC `measure (\(g,al).CARD (set (rules2Items (rules g)) DIFF (set al)))` THEN
 SRW_TAC [] [] THENL[
 (*1*)
-`!e.MEM e (rmDupes (v2::v3)) ==> MEM e (iclosure1 g (rmDupes (v2::v3)))` by 
+`∀e.MEM e (rmDupes (v2::v3)) ⇒ MEM e (iclosure1 g (rmDupes (v2::v3)))` by 
 METIS_TAC [iclosure1_mem] THEN
-`!e.MEM e (iclosure1 g (rmDupes (v2::v3))) ==> MEM e (rmDupes (iclosure1 g (rmDupes (v2::v3))))` 
+`∀e.MEM e (iclosure1 g (rmDupes (v2::v3))) ⇒ 
+		    MEM e (rmDupes (iclosure1 g (rmDupes (v2::v3))))` 
 by  METIS_TAC [rmd_r2] THEN
-`!e.MEM e (rmDupes (v2::v3)) ==> MEM e (rmDupes (iclosure1 g (rmDupes (v2::v3))))` by METIS_TAC []
+`∀e.MEM e (rmDupes (v2::v3)) ⇒ MEM e (rmDupes (iclosure1 g (rmDupes (v2::v3))))` 
+		    by METIS_TAC []
 THEN
 `LENGTH (rmDupes (iclosure1 g (rmDupes (v2::v3)))) >= LENGTH (rmDupes (v2::v3))` by
 METIS_TAC [mem_subset_len] THEN
-`CARD (set (rmDupes (iclosure1 g (rmDupes (v2::v3))))) >= CARD (set (rmDupes (v2::v3)))`  by 
+`CARD (set (rmDupes (iclosure1 g (rmDupes (v2::v3))))) >= 
+		    CARD (set (rmDupes (v2::v3)))`  by 
 METIS_TAC [list_set_len, rmDupes_twice] THEN
-`!e.MEM e (rmDupes (v2::v3)) ==> MEM e (iclosure1 g (rmDupes (v2::v3)))` by 
+`∀e.MEM e (rmDupes (v2::v3)) ⇒ MEM e (iclosure1 g (rmDupes (v2::v3)))` by 
 METIS_TAC [iclosure1_mem] THEN
 `(set (v2::v3)) SUBSET (set (iclosure1 g (rmDupes (v2::v3))))` by  
 METIS_TAC [mem_subset, rmDupes_lts] THEN
 `CARD (set (iclosure1 g (rmDupes (v2::v3)))) > CARD (v2 INSERT set v3)` by 
 METIS_TAC [set_neq_len, iclosure1_mem, FINITE_LIST_TO_SET, mem_subset, LIST_TO_SET_THM, rmDupes_lts] THEN
-`?e.e IN (set (iclosure1 g (rmDupes (v2::v3)))) /\ ~(e IN (v2 INSERT set v3))` by
+`∃e.e IN (set (iclosure1 g (rmDupes (v2::v3)))) ∧ ~(e IN (v2 INSERT set v3))` by
 METIS_TAC [set_neq, FINITE_LIST_TO_SET, rmDupes_lts, LIST_TO_SET_THM] THEN
 `MEM e (iclosure1 g (rmDupes (v2::v3)))` by FULL_SIMP_TAC (srw_ss()) [MEM_SET_TO_LIST] THEN
 `~(MEM e (v2::v3))` by FULL_SIMP_TAC (srw_ss()) [MEM_SET_TO_LIST] THEN
@@ -183,23 +203,23 @@ METIS_TAC [iclosure1_before_after_len, LIST_TO_SET_THM, rmDupes_lts] THEN
 FULL_SIMP_TAC (arith_ss) [],
 
 (*2*)
-`!e.MEM e (rmDupes (v2::v3)) ==> MEM e (iclosure1 g (rmDupes (v2::v3)))` by 
+`∀e.MEM e (rmDupes (v2::v3)) ⇒ MEM e (iclosure1 g (rmDupes (v2::v3)))` by 
 METIS_TAC [iclosure1_mem] THEN
-`!e.MEM e (iclosure1 g (rmDupes (v2::v3))) ==> MEM e (rmDupes (iclosure1 g (rmDupes (v2::v3))))` 
+`∀e.MEM e (iclosure1 g (rmDupes (v2::v3))) ⇒ MEM e (rmDupes (iclosure1 g (rmDupes (v2::v3))))` 
 by  METIS_TAC [rmd_r2] THEN
-`!e.MEM e (rmDupes (v2::v3)) ==> MEM e (rmDupes (iclosure1 g (rmDupes (v2::v3))))` by METIS_TAC []
+`∀e.MEM e (rmDupes (v2::v3)) ⇒ MEM e (rmDupes (iclosure1 g (rmDupes (v2::v3))))` by METIS_TAC []
 THEN
 `LENGTH (rmDupes (iclosure1 g (rmDupes (v2::v3)))) >= LENGTH (rmDupes (v2::v3))` by
 METIS_TAC [mem_subset_len] THEN
 `CARD (set (rmDupes (iclosure1 g (rmDupes (v2::v3))))) >= CARD (set (rmDupes (v2::v3)))`  by 
 METIS_TAC [list_set_len, rmDupes_twice] THEN
-`!e.MEM e (rmDupes (v2::v3)) ==> MEM e (iclosure1 g (rmDupes (v2::v3)))` 
+`∀e.MEM e (rmDupes (v2::v3)) ⇒ MEM e (iclosure1 g (rmDupes (v2::v3)))` 
 by METIS_TAC [iclosure1_mem] THEN
 `(set (v2::v3)) SUBSET (set (iclosure1 g (rmDupes (v2::v3))))` by  
 METIS_TAC [mem_subset, rmDupes_twice, LIST_TO_SET_THM, FINITE_LIST_TO_SET, rmDupes_lts] THEN
 `CARD (set (iclosure1 g (rmDupes (v2::v3)))) > CARD (v2 INSERT set v3)` by 
 METIS_TAC [set_neq_len, iclosure1_mem, FINITE_LIST_TO_SET, LIST_TO_SET_THM, rmDupes_lts] THEN
-`?e.e IN (set (iclosure1 g (rmDupes (v2::v3)))) /\ ~(e IN (v2 INSERT set v3))` by
+`∃e.e IN (set (iclosure1 g (rmDupes (v2::v3)))) ∧ ~(e IN (v2 INSERT set v3))` by
 METIS_TAC [set_neq, FINITE_LIST_TO_SET, rmDupes_lts, LIST_TO_SET_THM] THEN
 `MEM e (iclosure1 g (rmDupes (v2::v3)))` by FULL_SIMP_TAC (srw_ss()) [MEM_SET_TO_LIST] THEN
 `~(MEM e (v2::v3))` by FULL_SIMP_TAC (srw_ss()) [MEM_SET_TO_LIST, rmd_r2_1] THEN
@@ -207,53 +227,51 @@ METIS_TAC [set_neq, FINITE_LIST_TO_SET, rmDupes_lts, LIST_TO_SET_THM] THEN
 `e IN (set (rules2Items (rules g)))` by FULL_SIMP_TAC (srw_ss()) [] THEN
 `~(e IN (v2 INSERT set v3))`  by FULL_SIMP_TAC (srw_ss()) [] THEN
 `CARD (set (rules2Items (rules g))) - CARD (set (rules2Items (rules g)) INTER (v2 INSERT set v3)) > 0` by METIS_TAC [inter_card_less, FINITE_LIST_TO_SET] THEN
-FULL_SIMP_TAC (arith_ss) []])
+FULL_SIMP_TAC (arith_ss) []]);
 
 
-val _ = save_thm ("iclosure",iclosure)
-val _ = save_thm ("iclosure_ind",iclosure_ind)
+val _ = save_thm ("iclosure",iclosure);
+val _ = save_thm ("iclosure_ind",iclosure_ind);
 
 val iclosure_nil = store_thm ("iclosure_nil", 
-``!g l.~(l=[]) ==> ~(iclosure g l = [])``,
+``∀g l.~(l=[]) ⇒ ~(iclosure g l = [])``,
 HO_MATCH_MP_TAC iclosure_ind THEN SRW_TAC [] [] THEN
 SRW_TAC [] [iclosure, LET_THM] THEN
-METIS_TAC [iclosure1_not_nil, rmDupes_not_nil, len_not_0, LENGTH_NIL])
-
-
+METIS_TAC [iclosure1_not_nil, rmDupes_not_nil, len_not_0, LENGTH_NIL]);
 
 
 val auggr = Define `(auggr g s eof = 	
-         if ((~((NTS s) IN (nonTerminalsML g)) /\ 
+         if ((~((NTS s) IN (nonTerminalsML g)) ∧ 
 	    (~ ((TS eof) IN (terminalsML g))))) then 
          SOME (G ([(rule s [NTS (startSym g); TS eof])]++(rules g)) s) 
-         else NONE)`
+         else NONE)`;
 
 
 
 
 val lastEof = store_thm ("lastEof",
-``!g st eof.(auggr g st eof = SOME ag) ==> 
-  !l.RTC (rderives ag) [NTS (startSym ag)] (pfx++[NTS N]++sfx) ==> ~(N=startSym ag)
-  ==> ?pfx'.(sfx = pfx'++[TS eof])``,
+``∀g st eof.(auggr g st eof = SOME ag) ⇒ 
+  ∀l.RTC (rderives ag) [NTS (startSym ag)] (pfx++[NTS N]++sfx) ⇒ ~(N=startSym ag)
+  ⇒ ∃pfx'.(sfx = pfx'++[TS eof])``,
 SRW_TAC [] [auggr, LET_THM] THEN
 FULL_SIMP_TAC (srw_ss()) [startSym_def] THEN
 FULL_SIMP_TAC (srw_ss()) [Once RTC_CASES1, lreseq, rderives_def] THEN
 FULL_SIMP_TAC (srw_ss()) [rules_def] THENL[
 SRW_TAC [] [] THEN
-`?pfx'.(pfx ++ [NTS N] ++ sfx)=pfx'++[TS eof]` by METIS_TAC [rtcRderivesLastTmnl, APPEND] THEN
+`∃pfx'.(pfx ++ [NTS N] ++ sfx)=pfx'++[TS eof]` by METIS_TAC [rtcRderivesLastTmnl, APPEND] THEN
 Cases_on `sfx` THEN FULL_SIMP_TAC (srw_ss()) [] THENL[
 `NTS N = TS eof` by METIS_TAC [last_elem] THEN FULL_SIMP_TAC (srw_ss()) [],
 METIS_TAC [lastListBdown, NOT_CONS_NIL, last_append, last_elem]],
-METIS_TAC [slemma1_4, nonTerminalsEq]])
+METIS_TAC [slemma1_4, nonTerminalsEq]]);
 
 
 val auggr_startSym = store_thm ("auggr_startSym", 
-``(auggr g st eof = SOME ag) ==> (startSym ag = st)``,
-SRW_TAC [] [auggr] THEN SRW_TAC [] [startSym_def])
+``(auggr g st eof = SOME ag) ⇒ (startSym ag = st)``,
+SRW_TAC [] [auggr] THEN SRW_TAC [] [startSym_def]);
 
 
 val auggr_not_rd_nts = store_thm ("auggr_not_rd_nts",
-``!g st eof N.(auggr g st eof = SOME ag) ==> ~(N=st) ==> 
+``∀g st eof N.(auggr g st eof = SOME ag) ⇒ ~(N=st) ⇒ 
 ~ (RTC (rderives ag) [NTS (startSym ag)] [NTS N])``,
 SRW_TAC [] [Once RTC_CASES1] THENL[
 METIS_TAC [auggr_startSym],
@@ -270,13 +288,13 @@ Cases_on `RTC (rderives (G (rule st [NTS (startSym g); TS eof]::rules g) st))
 `MEM (TS eof) [NTS N]` by METIS_TAC [rtc_rderives_has_tmnl] THEN
 FULL_SIMP_TAC (srw_ss()) [],
 FULL_SIMP_TAC (srw_ss()) []],
-METIS_TAC [slemma1_4, nonTerminalsEq]]])
+METIS_TAC [slemma1_4, nonTerminalsEq]]]);
 
 
 val auggr_eq_start_rule = store_thm ("auggr_eq_start_rule",
-``!g st eof N r1 h.(auggr g st eof = SOME ag) ==> 
-(MEM (rule st (r1 ++ [h])) (rules ag)) ==> 
-((r1=[NTS (startSym g)]) /\ (h=TS eof))``,
+``∀g st eof N r1 h.(auggr g st eof = SOME ag) ⇒ 
+(MEM (rule st (r1 ++ [h])) (rules ag)) ⇒ 
+((r1=[NTS (startSym g)]) ∧ (h=TS eof))``,
 SRW_TAC [] [] THEN
 FULL_SIMP_TAC (srw_ss()) [auggr, LET_THM] THEN
 Cases_on `~(NTS st IN nonTerminalsML g)` THEN 
@@ -288,25 +306,25 @@ Cases_on `t` THEN SRW_TAC [] [] THEN FULL_SIMP_TAC (srw_ss()) [isNonTmnlSym_def,
 METIS_TAC [slemma1_4, nonTerminalsEq],
 Cases_on `r1` THEN SRW_TAC [] [] THEN FULL_SIMP_TAC (srw_ss()) [isNonTmnlSym_def, isTmnlSym_def] THEN
 Cases_on `t` THEN SRW_TAC [] [] THEN FULL_SIMP_TAC (srw_ss()) [isNonTmnlSym_def, isTmnlSym_def],
-METIS_TAC [slemma1_4, nonTerminalsEq]])
+METIS_TAC [slemma1_4, nonTerminalsEq]]);
 
 
 
 val auggrStartRule = store_thm ("auggrStartRule", 
-``!g st eof h.(auggr g st eof = SOME ag) 
-  ==> MEM (rule (startSym ag) h) (rules ag)
-  ==> (h=[NTS (startSym g);TS eof])``,
+``∀g st eof h.(auggr g st eof = SOME ag) 
+  ⇒ MEM (rule (startSym ag) h) (rules ag)
+  ⇒ (h=[NTS (startSym g);TS eof])``,
 SRW_TAC [] [auggr, LET_THM] THEN
 FULL_SIMP_TAC (srw_ss()) [startSym_def, rules_def] THEN
-METIS_TAC [slemma1_4, nonTerminalsEq])
+METIS_TAC [slemma1_4, nonTerminalsEq]);
 
 
 val auggrNotStInRtcRderives = store_thm ("auggrNotStInRtcRderives",
-``!u v.RTC (rderives ag) u v ==> (u=[NTS (startSym g); TS eof]) ==> 
-(auggr g st eof = SOME ag) ==> ~(MEM (NTS (startSym ag)) v)``,
+``∀u v.RTC (rderives ag) u v ⇒ (u=[NTS (startSym g); TS eof]) ⇒ 
+(auggr g st eof = SOME ag) ⇒ ~(MEM (NTS (startSym ag)) v)``,
 HO_MATCH_MP_TAC RTC_STRONG_INDUCT_RIGHT1 THEN SRW_TAC [] [RTC_RULES] THEN
 FULL_SIMP_TAC (srw_ss()) [auggr, LET_THM] THEN
-Cases_on `~(NTS st IN nonTerminalsML g) /\ ~(TS eof IN terminalsML g)` THEN 
+Cases_on `~(NTS st IN nonTerminalsML g) ∧ ~(TS eof IN terminalsML g)` THEN 
 FULL_SIMP_TAC (srw_ss()) [] THEN
 FULL_SIMP_TAC (srw_ss()) [] THENL[
 METIS_TAC [nonTerminalsEq, slemma1_4, startSym_def],
@@ -314,56 +332,56 @@ RES_TAC THEN
 FULL_SIMP_TAC (srw_ss()) [rderives_def] THEN
 SRW_TAC [] [] THEN
 FULL_SIMP_TAC (srw_ss()) [startSym_def, rules_def] THEN
-METIS_TAC [slemma1_4, nonTerminalsEq, startSym_def, rgr_r9eq]])
+METIS_TAC [slemma1_4, nonTerminalsEq, startSym_def, rgr_r9eq]]);
 
 
 val auggrStRtcDerivesSt = store_thm ("auggrStRtcDerivesSt",
-``!u v.RTC (rderives ag) u v ==> (u=[NTS (startSym ag)]) ==> 
-  (auggr g st eof = SOME ag) ==> ((v=[NTS (startSym ag)]) \/ ~(MEM (NTS (startSym ag)) v))``,
+``∀u v.RTC (rderives ag) u v ⇒ (u=[NTS (startSym ag)]) ⇒ 
+  (auggr g st eof = SOME ag) ⇒ ((v=[NTS (startSym ag)]) ∨ ~(MEM (NTS (startSym ag)) v))``,
 HO_MATCH_MP_TAC RTC_STRONG_INDUCT THEN SRW_TAC [] [RTC_RULES] THEN
 FULL_SIMP_TAC (srw_ss()) [rderives_def, lreseq] THEN
 SRW_TAC [] [] THEN
 `u'=[NTS (startSym g); TS eof]` by METIS_TAC [auggrStartRule] THEN
 SRW_TAC [] [] THEN
 FULL_SIMP_TAC (srw_ss()) [] THEN
-METIS_TAC [auggrNotStInRtcRderives])
+METIS_TAC [auggrNotStInRtcRderives]);
 
 
 val auggrRtcRderivesPfxSfxNil = store_thm ("auggrRtcRderivesPfxSfxNil",
-``!e pfx sfx.(auggr g st eof = SOME ag) ==>
-RTC (rderives ag) [NTS (startSym ag)] (pfx++[NTS (startSym ag)]++sfx) ==> 
-(pfx=[]) /\ (sfx=[])``,
+``∀e pfx sfx.(auggr g st eof = SOME ag) ⇒
+RTC (rderives ag) [NTS (startSym ag)] (pfx++[NTS (startSym ag)]++sfx) ⇒ 
+(pfx=[]) ∧ (sfx=[])``,
 SRW_TAC [] [] THEN
-`(pfx ++ [NTS (startSym ag)] ++ sfx = [NTS (startSym ag)]) \/ 
+`(pfx ++ [NTS (startSym ag)] ++ sfx = [NTS (startSym ag)]) ∨ 
 ~(MEM (NTS (startSym ag)) (pfx ++ [NTS (startSym ag)] ++ sfx))` by METIS_TAC [auggrStRtcDerivesSt] THEN
-FULL_SIMP_TAC (srw_ss()) [lreseq])
+FULL_SIMP_TAC (srw_ss()) [lreseq]);
 
 val auggrRtcRderivesStartRule = store_thm ("auggrRtcRderivesStartRule",
-``!u v.RTC (rderives ag) u v ==> (u=[NTS (startSym ag)])  ==> 
-      (auggr g st eof = SOME ag) ==>  
-     ~(v=[NTS (startSym ag)]) ==> RTC (rderives ag)  [NTS (startSym g); TS eof] v``,
+``∀u v.RTC (rderives ag) u v ⇒ (u=[NTS (startSym ag)])  ⇒ 
+      (auggr g st eof = SOME ag) ⇒  
+     ~(v=[NTS (startSym ag)]) ⇒ RTC (rderives ag)  [NTS (startSym g); TS eof] v``,
 HO_MATCH_MP_TAC RTC_STRONG_INDUCT THEN SRW_TAC [] [RTC_RULES] THEN
 FULL_SIMP_TAC (srw_ss()) [] THEN
-`!h.MEM (rule (startSym ag) h) (rules ag) ==>
+`∀h.MEM (rule (startSym ag) h) (rules ag) ⇒
          (h = [NTS (startSym g); TS eof])` by METIS_TAC [auggrStartRule] THEN
 FULL_SIMP_TAC (srw_ss()) [rderives_def, lreseq] THEN
 SRW_TAC [] [] THEN
 RES_TAC THEN
-FULL_SIMP_TAC (srw_ss()) [])
+FULL_SIMP_TAC (srw_ss()) []);
 
 val auggrDerivesNotNil = store_thm ("auggrDerivesNotNil",
-``!g st eof.
-            (auggr g st eof = SOME ag) ==>
-            !l.
-              RTC (rderives ag) [NTS (startSym ag)] (pfx ++ [NTS N] ++ sfx) ==>
-              ~(N = startSym ag) ==> ~(sfx=[])``,
+``∀g st eof.
+            (auggr g st eof = SOME ag) ⇒
+            ∀l.
+              RTC (rderives ag) [NTS (startSym ag)] (pfx ++ [NTS N] ++ sfx) ⇒
+              ~(N = startSym ag) ⇒ ~(sfx=[])``,
 SRW_TAC [] [] THEN
-`?pfx'. sfx = pfx' ++ [TS eof]` by METIS_TAC [lastEof] THEN
-FULL_SIMP_TAC (srw_ss()) [])
+`∃pfx'. sfx = pfx' ++ [TS eof]` by METIS_TAC [lastEof] THEN
+FULL_SIMP_TAC (srw_ss()) []);
 
 
 val auggrStRtcRderivesNotNil = store_thm ("auggrStRtcRderivesNotNil",
-``(auggr g st eof = SOME ag) ==> ~RTC (rderives ag) [NTS (startSym ag)] []``,
+``(auggr g st eof = SOME ag) ⇒ ~RTC (rderives ag) [NTS (startSym ag)] []``,
 SRW_TAC [] [Once RTC_CASES1] THEN
 Cases_on `~rderives ag [NTS (startSym ag)] u` THEN SRW_TAC [] [] THEN
 FULL_SIMP_TAC (srw_ss()) [rderives_def, lreseq] THEN
@@ -372,10 +390,10 @@ SRW_TAC [] [] THEN
 SRW_TAC [] [] THEN
 `MEM (TS eof)  [NTS (startSym g); TS eof]` by SRW_TAC [] [] THEN
 Cases_on `RTC (rderives ag) [NTS (startSym g); TS eof] []` THEN SRW_TAC [] [] THEN
-METIS_TAC [rgr_r9eq, MEM, MEM_APPEND, APPEND, rtc_rderives_has_tmnl])
+METIS_TAC [rgr_r9eq, MEM, MEM_APPEND, APPEND, rtc_rderives_has_tmnl]);
 
 val auggrRtcRderivesSt = store_thm ("auggrRtcRderivesSt",
-``(auggr g st eof = SOME ag) ==> RTC (rderives ag) [NTS (startSym ag)] [NTS lhs] ==> (lhs=startSym ag)``,
+``(auggr g st eof = SOME ag) ⇒ RTC (rderives ag) [NTS (startSym ag)] [NTS lhs] ⇒ (lhs=startSym ag)``,
 SRW_TAC [] [Once RTC_CASES1] THEN SRW_TAC [] [] THEN
 FULL_SIMP_TAC (srw_ss()) [rderives_def, lreseq] THEN
 SRW_TAC [] [] THEN
@@ -383,47 +401,46 @@ SRW_TAC [] [] THEN
 SRW_TAC [] [] THEN
 `MEM (TS eof)  [NTS (startSym g); TS eof]` by SRW_TAC [] [] THEN
 `MEM (TS eof) [NTS lhs]` by METIS_TAC [rgr_r9eq, MEM, MEM_APPEND, APPEND, rtc_rderives_has_tmnl] THEN
-FULL_SIMP_TAC (srw_ss()) [])
+FULL_SIMP_TAC (srw_ss()) []);
+
 
 val auggrStNotInRhs = store_thm ("auggrStNotInRhs",
-``(auggr g st eof = SOME ag) ==>
-  ~(?lhs rhs p s.MEM (rule lhs (p++[NTS (startSym ag)]++s)) 
+``(auggr g st eof = SOME ag) ⇒
+  ~(∃lhs rhs p s.MEM (rule lhs (p++[NTS (startSym ag)]++s)) 
    (rules ag))``,
 SRW_TAC [] [auggr, LET_THM, startSym_def, rules_def] THEN
-`~(?rhs.
-    MEM (rule st rhs) (rules g) \/
-   ?l p s.
-    MEM (rule l (p ++ [NTS st] ++ s)) (rules g) \/ 
+`~(∃rhs.
+    MEM (rule st rhs) (rules g) ∨
+   ∃l p s.
+    MEM (rule l (p ++ [NTS st] ++ s)) (rules g) ∨ 
    (st = startSym g))` by METIS_TAC [slemma1_4, nonTerminalsEq] THEN
 FULL_SIMP_TAC (srw_ss()) [startSym_def, rules_def] THEN
-Cases_on `~(lhs = st) \/ ~(p ++ [NTS st] ++ s = [NTS (startSym g); TS eof])` THEN
+Cases_on `~(lhs = st) ∨ ~(p ++ [NTS st] ++ s = [NTS (startSym g); TS eof])` THEN
 FULL_SIMP_TAC (srw_ss()) [] THEN
 Cases_on `p` THEN Cases_on `s` THEN FULL_SIMP_TAC (srw_ss()) []
 THENL[
       Cases_on `t` THEN FULL_SIMP_TAC (srw_ss()) [],
-      `LENGTH (t ++ [NTS st] ++ h'::t') = LENGTH [TS eof]` by METIS_TAC [] THEN
-      FULL_SIMP_TAC (srw_ss()) [] THEN
-      FULL_SIMP_TAC (arith_ss) []	    
-      ])
+      FULL_SIMP_TAC (srw_ss()) [lreseq]    
+      ]);
 
 
 
 val auggrNNeqSt = store_thm ("auggrNNeqSt",
-``!pfx sfx.RTC (rderives ag) [NTS (startSym ag)] 
-                             (pfx ++ [NTS N] ++ sfx) ==>
-  (auggr g st eof = SOME ag) ==>
-  (~(pfx=[]) \/ ~(sfx=[])) ==>
+``∀pfx sfx.RTC (rderives ag) [NTS (startSym ag)] 
+                             (pfx ++ [NTS N] ++ sfx) ⇒
+  (auggr g st eof = SOME ag) ⇒
+  (~(pfx=[]) ∨ ~(sfx=[])) ⇒
   ~(N=startSym ag)``,
 SRW_TAC [] [] THEN
 Cases_on `N=startSym ag` THEN
 FULL_SIMP_TAC (srw_ss()) [] THEN
-METIS_TAC [auggrStNotInRhs, rtcRderivesInRuleRhs])
+METIS_TAC [auggrStNotInRhs, rtcRderivesInRuleRhs]);
 
 
 
 val auggrStRtcRderivesSing = store_thm ("auggrStRtcRderivesSing", 
-``(auggr g st eof = SOME ag) ==>  (isTmnlSym h) ==> 
-RTC (rderives ag) [NTS (startSym ag)] [h] ==> (h=TS eof)``,
+``(auggr g st eof = SOME ag) ⇒  (isTmnlSym h) ⇒ 
+RTC (rderives ag) [NTS (startSym ag)] [h] ⇒ (h=TS eof)``,
 SRW_TAC [] [Once RTC_CASES2] THEN
 FULL_SIMP_TAC (srw_ss()) [isTmnlSym_def, rderives_def] THEN
 SRW_TAC [] [] THEN
@@ -434,7 +451,7 @@ THENL[
  THENL[
  METIS_TAC [auggrStartRule, NOT_CONS_NIL],
 
- `?pfx'.[TS s] = pfx'++[TS eof]` by METIS_TAC [lastEof, APPEND] THEN
+ `∃pfx'.[TS s] = pfx'++[TS eof]` by METIS_TAC [lastEof, APPEND] THEN
  `TS s = TS eof` by METIS_TAC [lastElemEq, APPEND_NIL] THEN
  FULL_SIMP_TAC (srw_ss()) []
  ],
@@ -445,7 +462,7 @@ THENL[
        `[TS s] = [NTS (startSym g); TS eof]` by METIS_TAC [auggrStartRule] THEN
        FULL_SIMP_TAC (srw_ss()) [],
 
-       `?pfx'.[] = pfx'++[TS eof]` by METIS_TAC [APPEND, NOT_CONS_NIL, lastEof, APPEND_NIL] THEN
+       `∃pfx'.[] = pfx'++[TS eof]` by METIS_TAC [APPEND, NOT_CONS_NIL, lastEof, APPEND_NIL] THEN
        Cases_on `pfx'` THEN FULL_SIMP_TAC (srw_ss()) []     
        ],
 
@@ -453,15 +470,15 @@ THENL[
  THENL[
  METIS_TAC [auggrStartRule, NOT_CONS_NIL],
 
- `?pfx'.[TS s] = pfx'++[TS eof]` by METIS_TAC [lastEof, APPEND] THEN
+ `∃pfx'.[TS s] = pfx'++[TS eof]` by METIS_TAC [lastEof, APPEND] THEN
  `TS s = TS eof` by METIS_TAC [lastElemEq, APPEND_NIL] THEN
  FULL_SIMP_TAC (srw_ss()) []
- ]])
+ ]]);
  
 val auggrAllTmsRhs = store_thm ("auggrAllTmsRhs",
-``(auggr g st eof = SOME ag) ==>
-   MEM (rule N rhs) (rules ag) ==>
-   EVERY isTmnlSym rhs ==>
+``(auggr g st eof = SOME ag) ⇒
+   MEM (rule N rhs) (rules ag) ⇒
+   EVERY isTmnlSym rhs ⇒
    ~(MEM (TS eof) rhs)``,			
 SRW_TAC [] [auggr, LET_THM, rules_def] THEN
 FULL_SIMP_TAC (srw_ss()) [rules_def]
@@ -472,31 +489,27 @@ THENL[
 
       Cases_on `~MEM (TS eof) rhs` THEN
       FULL_SIMP_TAC (srw_ss()) []  THEN
-      `~(?l p s. MEM (rule l (p ++ [TS eof] ++ s)) (rules g))` 
+      `~(∃l p s. MEM (rule l (p ++ [TS eof] ++ s)) (rules g))` 
        by METIS_TAC [terminalsEq, slemma1_4Tmnls] THEN
       METIS_TAC [rgr_r9eq]
-      ])
-
-
-
+      ]);
 
 
 val auggrEofInRhs = store_thm ("auggrEofInRhs",
-``(auggr g st eof = SOME ag) ==>
-  (MEM (rule lhs rhs) (rules ag)) ==>
-  MEM (TS eof) rhs ==>
+``(auggr g st eof = SOME ag) ⇒
+  (MEM (rule lhs rhs) (rules ag)) ⇒
+  MEM (TS eof) rhs ⇒
   (lhs = startSym ag)``,
 SRW_TAC [] [auggr, LET_THM] THEN
 FULL_SIMP_TAC (srw_ss()) [startSym_def, rules_def]THEN
-METIS_TAC [rgr_r9eq, slemma1_4Tmnls, terminalsEq]
-)
+METIS_TAC [rgr_r9eq, slemma1_4Tmnls, terminalsEq]);
 
 
 
 val auggrRtcRdLastSymEof = store_thm ("auggrRtcRdLastSymEof",
-``!u v.RTC (rderives ag) u v ==> (u=[NTS (startSym ag)]) ==>
-(auggr g st eof = SOME ag) ==>
-MEM (TS eof) v ==> 
+``∀u v.RTC (rderives ag) u v ⇒ (u=[NTS (startSym ag)]) ⇒
+(auggr g st eof = SOME ag) ⇒
+MEM (TS eof) v ⇒ 
 (LAST v = TS eof)``,
 HO_MATCH_MP_TAC RTC_STRONG_INDUCT_RIGHT1 THEN
 SRW_TAC [] [RTC_RULES] THEN
@@ -506,17 +519,11 @@ FULL_SIMP_TAC (srw_ss()) [MEM_APPEND]
 THENL[
       `(LAST (s1 ++ [NTS lhs] ++ s2) = TS eof)` by METIS_TAC [] THEN
       Cases_on `s2` THEN
-      FULL_SIMP_TAC (srw_ss()) []
-      THENL[
-	    `NTS lhs = TS eof` by METIS_TAC [last_elem] THEN
-	    FULL_SIMP_TAC (srw_ss()) [],
-
-	    METIS_TAC [last_append, NOT_CONS_NIL]
-	    ],
+      FULL_SIMP_TAC (srw_ss()) [],
 
       `lhs=startSym ag` by METIS_TAC [auggrEofInRhs] THEN
       SRW_TAC [] [] THEN
-      `(s1=[]) /\ (s2=[])`by METIS_TAC [auggrRtcRderivesPfxSfxNil] THEN
+      `(s1=[]) ∧ (s2=[])`by METIS_TAC [auggrRtcRderivesPfxSfxNil] THEN
       SRW_TAC [] [] THEN
       FULL_SIMP_TAC (srw_ss()) [] THEN
       `rhs=[NTS (startSym g); TS eof]` by METIS_TAC [auggrStartRule] THEN
@@ -525,25 +532,25 @@ THENL[
       Cases_on `s2` THEN
       FULL_SIMP_TAC (srw_ss()) [] THEN
       METIS_TAC [last_append, NOT_CONS_NIL]
-      ])
+      ]);
 
 
 
 
 val auggrNewRuleMem = 
 store_thm ("auggrNewRuleMem",
-``(auggr g st eof = SOME ag) ==>
+``(auggr g st eof = SOME ag) ⇒
 MEM (rule (startSym ag) [NTS (startSym g);TS eof]) (rules ag)``,
 SRW_TAC [][auggr,LET_THM] THEN
-FULL_SIMP_TAC (srw_ss()) [startSym_def,rules_def])
+FULL_SIMP_TAC (srw_ss()) [startSym_def,rules_def]);
 
 val auggrStNeqOSt =store_thm
 ("auggrStNeqOSt",
-``(auggr g st eof = SOME ag) ==>
+``(auggr g st eof = SOME ag) ⇒
   ~(startSym g = startSym ag)``,
 SRW_TAC [][] THEN
 FULL_SIMP_TAC (srw_ss()) [rderives_def,auggr,LET_THM] THEN
-Cases_on `~(NTS st IN nonTerminalsML g) /\
+Cases_on `~(NTS st IN nonTerminalsML g) ∧
              ~(TS eof IN terminalsML g)` THEN
 FULL_SIMP_TAC (srw_ss()) [] THEN
 SRW_TAC [][rules_def,startSym_def] THEN
@@ -551,39 +558,39 @@ FULL_SIMP_TAC (srw_ss()) []  THEN
 Cases_on `~(startSym g = st)` THEN
 SRW_TAC [][] THEN
 METIS_TAC [slemma1_4,nonTerminalsEq]
-)
+);
 
 val auggr_neqStartSym2 = store_thm ("auggr_neqStartSym2", 
-``(auggr g st eof = SOME ag) ==> 
-MEM (rule n l) (rules ag) ==> ~(LAST l = TS eof) ==> ~(n=st)``,
+``(auggr g st eof = SOME ag) ⇒ 
+MEM (rule n l) (rules ag) ⇒ ~(LAST l = TS eof) ⇒ ~(n=st)``,
 SRW_TAC [] [auggr] THEN
 FULL_SIMP_TAC (srw_ss()) [rules_def] THENL[
 METIS_TAC [last_elem, APPEND],
 Cases_on `n=st` THEN
-METIS_TAC [slemma1_4, nonTerminalsEq]])
+METIS_TAC [slemma1_4, nonTerminalsEq]]);
 
 
 val lang2rtc2list = store_thm ("lang2rtc2list",
-``(auggr g st eof = SOME ag) ==>
-  sl IN language ag ==>
+``(auggr g st eof = SOME ag) ⇒
+  sl IN language ag ⇒
   ((rderives ag [NTS (startSym ag)] [NTS (startSym g);TS eof]) 
-/\ ?dtl.
+∧ ∃dtl.
    rtc2list (rderives ag) (([NTS (startSym g);TS eof]) :: dtl)
-/\ ((LAST (([NTS (startSym g);TS eof])::dtl)) = sl) 
-/\ MEM (rule (startSym ag) ([NTS (startSym g);TS eof])) (rules ag))``,
+∧ ((LAST (([NTS (startSym g);TS eof])::dtl)) = sl) 
+∧ MEM (rule (startSym ag) ([NTS (startSym g);TS eof])) (rules ag))``,
 
 SRW_TAC [][] 
 THENL[
       FULL_SIMP_TAC (srw_ss()) [rderives_def,auggr,LET_THM] THEN
       Cases_on `~(NTS st IN nonTerminalsML g) 
-		/\~(TS eof IN terminalsML g)` THEN
+		∧~(TS eof IN terminalsML g)` THEN
       FULL_SIMP_TAC (srw_ss()) [] THEN
       SRW_TAC [][rules_def,startSym_def] THEN
       FULL_SIMP_TAC (srw_ss()) [] THEN
       METIS_TAC [APPEND_NIL,auggr_startSym,EVERY_DEF],
 
-      `?dl.rtc2list (rderives ag) dl /\
-       (HD dl = [NTS (startSym ag)]) /\ (LAST dl = sl)` 
+      `∃dl.rtc2list (rderives ag) dl ∧
+       (HD dl = [NTS (startSym ag)]) ∧ (LAST dl = sl)` 
 	  by METIS_TAC [rtc2list_exists,listderiv_def] THEN
       SRW_TAC [][] THEN
       Cases_on `dl` THEN
@@ -598,28 +605,30 @@ THENL[
       FULL_SIMP_TAC (srw_ss()) [] THEN
       Q.EXISTS_TAC `t'`THEN
       SRW_TAC [][]
-      ])
+      ]);
 
 val ag_new_rule = store_thm("ag_new_rule", 
-``!g s eof.(auggr g s eof = SOME ag)
-==> (MEM (rule s [NTS (startSym g);TS eof]) (rules ag) /\ (s=startSym ag))``,
+``∀g s eof.(auggr g s eof = SOME ag)
+⇒ (MEM (rule s [NTS (startSym g);TS eof]) (rules ag) ∧ (s=startSym ag))``,
 SRW_TAC [] [auggr, rules_def, MEM, startSym_def, APPEND, MEM_APPEND] THEN
-SRW_TAC [] [auggr, rules_def, MEM, startSym_def, APPEND, MEM_APPEND])
+SRW_TAC [] [auggr, rules_def, MEM, startSym_def, APPEND, MEM_APPEND]);
 
 
-val initProds2Items = Define `(initProds2Items s [] = []) /\
-(initProds2Items s ((rule l r)::rs) = if (s=l) then (((item l ([],r)))::initProds2Items s rs) else initProds2Items s rs)`
+val initProds2Items = Define 
+`(initProds2Items s [] = []) ∧
+(initProds2Items s ((rule l r)::rs) = 
+ if (s=l) then (((item l ([],r)))::initProds2Items s rs) else initProds2Items s rs)`;
 
 
 val auggrExistsMemInit = store_thm ("auggrExistsMemInit",
-``(auggr g s eof = SOME ag) ==> 
+``(auggr g s eof = SOME ag) ⇒ 
       MEM (item (startSym ag) ([],[NTS (startSym g);TS eof])) (initProds2Items (startSym ag) (rules ag))``,
 SRW_TAC [] [auggr, LET_THM, startSym_def, rules_def, initProds2Items] THEN
-SRW_TAC [] [startSym_def, rules_def, initProds2Items])
+SRW_TAC [] [startSym_def, rules_def, initProds2Items]);
 
 
 val initItems = Define
-(`(initItems g r = iclosure g (initProds2Items (startSym g) r))`)
+(`(initItems g r = iclosure g (initProds2Items (startSym g) r))`);
 (*
 Induct_on `r` THEN SRW_TAC [] [initItems, initProds2Items, iclosure] THEN
 Cases_on `h` THEN SRW_TAC [] [initItems, initProds2Items, iclosure] THEN
@@ -633,21 +642,21 @@ Cases_on `h` THEN SRW_TAC [] [initItems, initProds2Items, iclosure] THEN
 
 
 
- val moveDot = Define `(moveDot [] sym = []) /\
+ val moveDot = Define `(moveDot [] sym = []) ∧
  (moveDot ((item str (a,(s::ss)))::it) sym =  
-if (s=sym) then (item str (a++[s],ss))::moveDot it sym else moveDot it sym) /\
- (moveDot (_::it) sym = moveDot it sym)`
+if (s=sym) then (item str (a++[s],ss))::moveDot it sym else moveDot it sym) ∧
+ (moveDot (_::it) sym = moveDot it sym)`;
 
 val trans = Define
-`(trans ag (s,[]) = SOME s) /\
+`(trans ag (s,[]) = SOME s) ∧
  (trans ag (s,sym::rst) =
     case moveDot s sym of 
        [] -> NONE
-    || x -> trans ag (iclosure ag x, rst))`
+    || x -> trans ag (iclosure ag x, rst))`;
  
 
 val EXISTS_item = store_thm("EXISTS_item",
-  ``(?i:item. P i) = ?N p s. P (item N (p,s))``,
+  ``(∃i:('nts,'ts) item. P i) = ∃N p s. P (item N (p,s))``,
   SRW_TAC [][EQ_IMP_THM] THENL[
     Cases_on `i` THEN Cases_on `p` THEN METIS_TAC [],
     METIS_TAC []
@@ -657,14 +666,16 @@ val EXISTS_item = store_thm("EXISTS_item",
 
 val nextState = Define `nextState g itl sym = iclosure g (moveDot itl sym)`
 
-val validItl = Define `(validItl g [] = T) /\
-(validItl g (item l (r1,r2) :: rst) = MEM (rule l (r1++r2)) (rules g) /\ validItl g rst)`
+val validItl = Define 
+`(validItl g [] = T) ∧
+(validItl g (item l (r1,r2) :: rst) = 
+MEM (rule l (r1++r2)) (rules g) ∧ validItl g rst)`;
 
-val validStates = Define `(validStates g [] = T) /\
-(validStates g ((sym, itl)::rst) = validItl g itl /\ validStates g rst)`
+val validStates = Define `(validStates g [] = T) ∧
+(validStates g ((sym, itl)::rst) = validItl g itl ∧ validStates g rst)`;
 
 val validItl_append = store_thm ("validItl_append",
-``validItl g (l1++l2) = validItl g l1 /\ validItl g l2``,
+``validItl g (l1++l2) = validItl g l1 ∧ validItl g l2``,
 SRW_TAC [] [EQ_IMP_THM] THENL [
 Induct_on `l1` THEN SRW_TAC [] [] THEN FULL_SIMP_TAC (srw_ss()) [validItl] THEN 
 Cases_on `h` THEN Cases_on `p` THEN FULL_SIMP_TAC (srw_ss()) [validItl],
@@ -676,105 +687,110 @@ Induct_on `l2` THEN SRW_TAC [] [] THEN Induct_on `l1` THEN
 FULL_SIMP_TAC (srw_ss()) [validItl] THEN 
 SRW_TAC [] [] THEN Cases_on `h'` THEN 
 Cases_on `p` THEN FULL_SIMP_TAC (srw_ss()) [validItl]]
-)
+);
 
 
 val validStates_append = store_thm ("validStates_append", 
-``!l1 l2.validStates g (l1 ++ l2) = validStates g l1 /\ validStates g l2``,
+``∀l1 l2.validStates g (l1 ++ l2) = validStates g l1 ∧ validStates g l2``,
 Induct_on `l1` THEN Induct_on `l2` THEN SRW_TAC [] [validStates] THEN
-Cases_on `h'` THEN METIS_TAC [validStates, APPEND])
+Cases_on `h'` THEN METIS_TAC [validStates, APPEND]);
 
 
 val validStates_pop = store_thm ("validStates_pop", 
-``!g l n.validStates g l ==> validStates g (pop l n)``,
-METIS_TAC [popl, validStates_append])
+``∀g l n.validStates g l ⇒ validStates g (pop l n)``,
+METIS_TAC [popl, validStates_append]);
 
 val validItl_md = store_thm ("validItl_md",
-``!itl sym.validItl g itl ==> validItl g (moveDot itl sym)``,
+``∀itl sym.validItl g itl ⇒ validItl g (moveDot itl sym)``,
 Induct_on `itl` THEN SRW_TAC [] [validItl, moveDot] THEN
 Cases_on `h` THEN Cases_on `p` THEN Cases_on `r` THEN
 FULL_SIMP_TAC (srw_ss()) [validItl, moveDot] THEN
 Cases_on `h=sym` THEN SRW_TAC [] [validItl] THEN 
-METIS_TAC [APPEND, APPEND_ASSOC])
+METIS_TAC [APPEND, APPEND_ASSOC]);
 
 
 val validItl_rules_cons = store_thm ("validItl_rules_cons",
-``!r s l e.validItl (G r s) l ==> validItl (G (e::r) s) l``,
+``∀r s l e.validItl (G r s) l ⇒ validItl (G (e::r) s) l``,
 SRW_TAC [] [] THEN
 Induct_on `l` THEN SRW_TAC [] [validItl] THEN
-Cases_on `h` THEN Cases_on `p`  THEN FULL_SIMP_TAC (srw_ss()) [validItl, rules_def])
+Cases_on `h` THEN Cases_on `p`  THEN FULL_SIMP_TAC (srw_ss()) [validItl, rules_def]);
 
 
 val rules2items_sub2 = store_thm ("rules2items_sub2",
-``!g.validItl g  (rules2Items (rules g))``,
+``∀g.validItl g  (rules2Items (rules g))``,
 Cases_on `g` THEN SRW_TAC [] [rules_def] THEN
 Induct_on `l` THEN SRW_TAC [] [validItl, rules2Items] THEN
 Cases_on `h` THEN FULL_SIMP_TAC (srw_ss()) [validItl, rules_def, rules2Items] THEN
-METIS_TAC [validItl_rules_cons])
+METIS_TAC [validItl_rules_cons]);
 
 
 val validItl_mem = store_thm ("validItl_mem",
-``!l.validItl g l = (!e.MEM e l ==> validItl g [e])``,
+``∀l.validItl g l = (∀e.MEM e l ⇒ validItl g [e])``,
 Induct_on `l` THEN SRW_TAC [] [validItl, EQ_IMP_THM] THEN
-METIS_TAC [validItl_append, APPEND])
+METIS_TAC [validItl_append, APPEND]);
 
 
 
 val validItl_getItems = store_thm ("validItl_getItems",
-``! g sym.validItl g (getItems (rules g) sym)``,
-Induct_on `rules g` THEN SRW_TAC [] [validItl, getItems] THENL[
-METIS_TAC [validItl, getItems],
+``∀sym.validItl g (getItems (rules g) sym)``,
+
+Induct_on `rules g` THEN SRW_TAC [] [validItl, getItems] THEN1
+METIS_TAC [validItl, getItems] THEN
 `rules g = h::v` by METIS_TAC [] THEN 
 Cases_on `h` THEN ONCE_ASM_REWRITE_TAC [] THEN
-`!e.MEM e (getItems (rule s l::v) sym) ==> MEM e (rules2Items (rule s l::v))` by METIS_TAC [rules2items_sub] THEN
-`validItl g (rules2Items (rule s l ::v))` by METIS_TAC [rules2items_sub2, rules_def] THEN
-`!e.MEM e (rules2Items (rule s l::v)) ==> validItl g [e]` by METIS_TAC [validItl_mem] THEN
-METIS_TAC [validItl_mem, APPEND, validItl_append]])
+`∀e.MEM e (getItems (rule n l::v) sym) ⇒ MEM e (rules2Items (rule n l::v))` 
+				   by METIS_TAC [rules2items_sub] THEN
+`validItl g (rules2Items (rule n l ::v))` 
+by METIS_TAC [rules2items_sub2, rules_def,validItl] THEN
+`∀e.MEM e (rules2Items (rule n l::v)) ⇒ validItl g [e]` 
+				   by METIS_TAC [validItl_mem] THEN
+METIS_TAC [validItl_mem, APPEND, validItl_append]);
+
 
 val validItl_iclosure1 = store_thm ("validItl_iclosure1", 
-``!g itl.validItl g itl ==> validItl g (iclosure1 g itl)``,
+``∀g itl.validItl g itl ⇒ validItl g (iclosure1 g itl)``,
 Induct_on `itl` THEN SRW_TAC [] [validItl, iclosure1] THEN
 Cases_on `h` THEN Cases_on `p` THEN Cases_on `r` THEN
 FULL_SIMP_TAC (srw_ss()) [iclosure1, validItl] THEN
 Cases_on `h` THEN FULL_SIMP_TAC (srw_ss()) [iclosure1, validItl] THEN
-METIS_TAC [validItl, validItl_append, APPEND, APPEND_ASSOC, validItl_getItems])
+METIS_TAC [validItl, validItl_append, APPEND, APPEND_ASSOC, validItl_getItems]);
 
 
 val validItl_delete = store_thm ("validItl_delete",
-``!g t h.validItl g t ==> validItl g (delete h t)``,
+``∀g t h.validItl g t ⇒ validItl g (delete h t)``,
 Induct_on `t` THEN SRW_TAC [] [delete_def, validItl] THEN
-METIS_TAC [validItl_append, APPEND])
+METIS_TAC [validItl_append, APPEND]);
 
 
 val validItl_rmDupes = store_thm ("validItl_rmDupes", 
-``!itl.validItl g itl ==> validItl g (rmDupes itl)``,
+``∀itl.validItl g itl ⇒ validItl g (rmDupes itl)``,
 HO_MATCH_MP_TAC rmDupes_ind THEN SRW_TAC [] [rmDupes, validItl] THEN
-METIS_TAC [validItl_append, APPEND, validItl_delete])
+METIS_TAC [validItl_append, APPEND, validItl_delete]);
 
 
 val validItl_iclosure = store_thm ("validItl_iclosure",
-``!g itl.validItl g itl ==> validItl g (iclosure g itl)``,
+``∀g itl.validItl g itl ⇒ validItl g (iclosure g itl)``,
 HO_MATCH_MP_TAC iclosure_ind THEN SRW_TAC [] [iclosure, validItl, LET_THM] THEN
-METIS_TAC [validItl_rmDupes, validItl_iclosure1])
+METIS_TAC [validItl_rmDupes, validItl_iclosure1]);
 
-val sgoto = Define `sgoto g itl sym = nextState g itl sym`
+val sgoto = Define `sgoto g itl sym = nextState g itl sym`;
 
 
 val validItl_sgoto = store_thm ("validItl_sgoto", 
-``!g itl sym.validItl g itl ==> validItl g (sgoto g itl sym)``,
+``∀g itl sym.validItl g itl ⇒ validItl g (sgoto g itl sym)``,
 SRW_TAC [] [sgoto, nextState] THEN
 `validItl g (moveDot itl sym)` by METIS_TAC [validItl_md] THEN
-METIS_TAC [validItl_iclosure])
+METIS_TAC [validItl_iclosure]);
 
 
-
+(*!!!!Make followSet followSetML*)
 val reduce = Define `
-(reduce g [] s = []) /\ 
-(reduce g (item l (r, [])::it) s  = 
-if ((TS s) IN (followSetML g (NTS l))) then 
-    ((rule l r)::reduce g it s) else reduce g it s) /\
-(reduce g ((item l (r, _))::it) s = reduce g it s)`
-
+(reduce (g:(α,β) grammar) ([]:(α,β) item list) (s:β) = []:(α,β) rule list) ∧ 
+(reduce (g:(α,β) grammar) 
+(item (l:α) (r:(α,β) symbol list, []:(α,β) symbol list)::it) (s:β)  = 
+if ((TS s) IN (followSet g (NTS l))) then 
+    ((rule l r)::reduce g it s) else reduce g it s) ∧
+(reduce g ((item l (r, _))::it) s = reduce g it s)`;
 
 
 val buildTree = Define `(buildTree p r = 
@@ -783,14 +799,14 @@ val buildTree = Define `(buildTree p r =
 			     if (s=NONE) then NONE
 				 else
 				     if (r=THE s) then take (LENGTH r) (MAP SND p)
-					 else NONE)`
+					 else NONE)`;
 
 
 
 val addRule = Define `(addRule p (rule l r) = 
          let x =  buildTree p (REVERSE r) in 
               if (x = NONE) then NONE 
-	      else SOME  (Node l (REVERSE (THE x))))`
+	      else SOME  (Node l (REVERSE (THE x))))`;
 
 (* stack top is the first element *)
 (* ptree is a stack of parsetrees *)
@@ -802,7 +818,7 @@ nonterminal symbol -> goto or reduce -> both then conflict
 accept when all symbols read and only one parse tree exists
 *)
 
-val machine = Define `machine g = (sgoto g, reduce g)`
+val machine = Define `machine g = (sgoto g, reduce g)`;
 
 (* slr :: grammar -> machine option *)
 (* 
@@ -810,7 +826,7 @@ if reduce returns more than 1 rule -> NONE
 if reduce and goto are null -> NONE
 if both are not null and return different states -> NONE
 ----------------
-if ?itl1 itl2, sym IN grammar : sgoto g itl1 sym [] = itl2 /\ 
+if ∃itl1 itl2, sym IN grammar : sgoto g itl1 sym [] = itl2 ∧ 
 iclosure (reduce)
 *)
 
@@ -819,16 +835,16 @@ let
 sg = sgoto g and
 red = reduce g
 in
-if (?pfx itl sym.(trans g (initItems g (rules g),pfx) = SOME itl) /\
+if (∃pfx itl sym. isTmnlSym sym ∧ (trans g (initItems g (rules g),pfx) = SOME itl) ∧
 let
     (s = sg itl sym) and
-    (r = red itl (sym2Str sym))
+    (r = red itl (ts2str sym))
 in
 case (s,r) of (* ([],[]) dealt in the parser *)
  ((x::xs),(y::ys)) -> T
 || (_,(y::y'::ys)) -> T
 || otherwise -> F)
-then NONE else SOME (sg,red)`
+then NONE else SOME (sg,red)`;
 
 
 (*
@@ -841,106 +857,110 @@ then NONE else SOME (sg,red)`
 *)
 
 val ruleItems_defn = Hol_defn "ruleItems_defn" 
-`(ruleItems (item l (r,[])) = [item l (r,[])]) /\
-(ruleItems (item l ([],x::xs)) = item l ([],x::xs) :: ruleItems (item l ([x],xs))) /\
-(ruleItems (item l (r1,x::xs))  = item l (r1,x::xs) :: ruleItems (item l (r1++[x],xs)))`
+`(ruleItems (item l (r,[])) = [item l (r,[])]) ∧
+(ruleItems (item l ([],x::xs)) = item l ([],x::xs) :: ruleItems (item l ([x],xs))) ∧
+(ruleItems (item l (r1,x::xs))  = 
+ item l (r1,x::xs) :: ruleItems (item l (r1++[x],xs)))`;
 
-val itemPair = Define `itemPair (item l x) = x`
+val itemPair = Define `itemPair (item l x) = x`;
 
 
 val (ruleItems, ruleItems_ind) = tprove (ruleItems_defn,
-WF_REL_TAC `measure (\x.(LENGTH (SND (itemPair x))))` THEN SRW_TAC [] [itemPair, SND])
+WF_REL_TAC `measure (\x.(LENGTH (SND (itemPair x))))` THEN 
+SRW_TAC [] [itemPair, SND]);
 
-val allItems = Define `(allItems [] = []) /\
-(allItems (rule l r::rs) = ruleItems (item l ([], r)) ++ allItems rs)`
+val allItems = Define `(allItems [] = []) ∧
+(allItems (rule l r::rs) = ruleItems (item l ([], r)) ++ allItems rs)`;
 
-val symNeighbour = Define `(symNeighbour g itl sym = rmDupes (iclosure g (moveDot itl sym)))`
+val symNeighbour = Define 
+`(symNeighbour g itl sym = rmDupes (iclosure g (moveDot itl sym)))`;
 
-val asNeighbours = Define `(asNeighbours g itl [] = []) /\
-(asNeighbours g itl (x::xs) =  (symNeighbour g itl x::asNeighbours g itl xs))`
+val asNeighbours = Define `(asNeighbours g itl [] = []) ∧
+(asNeighbours g itl (x::xs) =  (symNeighbour g itl x::asNeighbours g itl xs))`;
 
 
 val visit_defn = Hol_defn "visit_defn" 
 `(visit g sn itl = 
-if ~(ALL_DISTINCT itl) \/ ~(validItl g itl) then [] else
+if ~(ALL_DISTINCT itl) ∨ ~(validItl g itl) then [] else
 let 
 s = asNeighbours g itl (SET_TO_LIST (allSyms g)) 
 in
 		     let
 			 rem = diff s sn
 		     in
-			 rem++(FLAT (MAP (visit g (sn++rem)) rem)))`
+			 rem++(FLAT (MAP (visit g (sn++rem)) rem)))`;
 
 val itemEqRule = Define 
-`itemEqRule g (item l (r1,r2)) = MEM (rule l (r1++r2)) (rules g)`
+`itemEqRule g (item l (r1,r2)) = MEM (rule l (r1++r2)) (rules g)`;
 
-val isGrammarItl = Define `(isGrammarItl g itl = EVERY (itemEqRule g) itl)`
+val isGrammarItl = Define `(isGrammarItl g itl = EVERY (itemEqRule g) itl)`;
 
 val allGrammarItls = Define 
-`allGrammarItls g = {itl | isGrammarItl g itl /\ ALL_DISTINCT itl}`
+`allGrammarItls g = {itl | isGrammarItl g itl ∧ ALL_DISTINCT itl}`;
 
 val finite_allItems = store_thm ("finite_allItems",
-``!g.FINITE {i|MEM i (allItems (rules g))}``,
-`!g.{i|MEM i (allItems (rules g))} = {i|i IN LIST_TO_SET (allItems (rules g))}` by METIS_TAC [setc_mem_in] THEN
-SRW_TAC [] [EXTENSION])
+``∀g.FINITE {i|MEM i (allItems (rules g))}``,
+`∀g.{i|MEM i (allItems (rules g))} = 
+{i|i IN LIST_TO_SET (allItems (rules g))}` by METIS_TAC [setc_mem_in] THEN
+SRW_TAC [] [EXTENSION]);
 
 val itemEqRuleRulesEqGrRules = store_thm ("itemEqRuleRulesEqGrRules",
-``!g.{rule l (r1++r2) | itemEqRule g (item l (r1,r2))} = (LIST_TO_SET (rules g))``,
+``∀g.{rule l (r1++r2) | itemEqRule g (item l (r1,r2))} = (LIST_TO_SET (rules g))``,
 SRW_TAC [] [itemEqRule, SUBSET_DEF, EQ_IMP_THM, EXTENSION] THENL[
 METIS_TAC [],
 Cases_on `x` THEN Induct_on `l` THEN SRW_TAC [] [] THEN
- METIS_TAC [APPEND]])
+ METIS_TAC [APPEND]]);
 
 val allItems_append = store_thm ("allItems_append",
-``!l1 l2.allItems (l1++l2) = allItems l1 ++ allItems l2``,
+``∀l1 l2.allItems (l1++l2) = allItems l1 ++ allItems l2``,
 Induct_on `l1` THEN Induct_on `l2` THEN SRW_TAC [] [allItems] THEN
 Cases_on `h` THEN Cases_on `h'` THEN METIS_TAC [APPEND, APPEND_ASSOC, allItems]
-)
+);
     
 
-val itemLhs = Define `itemLhs (item l r) = l`
-val itemFstRhs = Define `itemFstRhs (item l r) = FST r`
-val itemSndRhs = Define `itemSndRhs (item l r) = SND r`
+val itemLhs = Define `itemLhs (item l r) = l`;
+val itemFstRhs = Define `itemFstRhs (item l r) = FST r`;
+val itemSndRhs = Define `itemSndRhs (item l r) = SND r`;
 
 val ruleItems_mem = store_thm ("ruleItems_mem",
-``!it.MEM (item (itemLhs it) (itemFstRhs it++itemSndRhs it,[])) (ruleItems it)``,
+``∀it.MEM (item (itemLhs it) (itemFstRhs it++itemSndRhs it,[])) (ruleItems it)``,
 HO_MATCH_MP_TAC ruleItems_ind THEN SRW_TAC [] [] THEN
 FULL_SIMP_TAC (srw_ss()) [ruleItems, itemLhs, itemFstRhs, itemSndRhs] THEN
-METIS_TAC [APPEND, APPEND_ASSOC])
+METIS_TAC [APPEND, APPEND_ASSOC]);
 
 val allMemRuleItems = store_thm ("allMemRuleItems",
-``!it r1 r2.(itemSndRhs it = r1++r2) ==> MEM (item (itemLhs it) (itemFstRhs it++r1,r2)) (ruleItems it)``,
+``∀it r1 r2.(itemSndRhs it = r1++r2) ⇒ MEM (item (itemLhs it) (itemFstRhs it++r1,r2)) (ruleItems it)``,
 HO_MATCH_MP_TAC ruleItems_ind THEN SRW_TAC [] [ruleItems, itemFstRhs, itemSndRhs, itemLhs] THEN
-Induct_on `r1` THEN SRW_TAC [] [] THEN METIS_TAC [APPEND, APPEND_NIL, APPEND_ASSOC])
+Induct_on `r1` THEN SRW_TAC [] [] THEN METIS_TAC [APPEND, APPEND_NIL, APPEND_ASSOC]);
 
 
 val memRuleAllItems = store_thm ("memRuleAllItems",
-``!l r rs.MEM (rule l r) rs ==> !r1 r2.(r=r1++r2) ==> MEM (item l (r1,r2)) (allItems rs)``,
+``∀l r rs.MEM (rule l r) rs ⇒ ∀r1 r2.(r=r1++r2) ⇒ MEM (item l (r1,r2)) (allItems rs)``,
 Induct_on `rs` THEN SRW_TAC [] [] THEN FULL_SIMP_TAC (srw_ss()) [allItems] THENL[
 `MEM (item (itemLhs (item l ([],r1++r2))) (itemFstRhs (item l ([],r1++r2)) ++r1,r2)) (ruleItems (item l ([],r1++r2)))`
 by FULL_SIMP_TAC (srw_ss()) [allMemRuleItems, itemSndRhs] THEN
 FULL_SIMP_TAC (srw_ss()) [itemFstRhs, itemLhs, itemSndRhs],
-Cases_on `h` THEN SRW_TAC [] [allItems]])
+Cases_on `h` THEN SRW_TAC [] [allItems]]);
 
 
 val itemEqRuleExists = store_thm ("itemEqRuleExists",
- ``!it.!s q r.MEM (item s (q,r)) (ruleItems it) ==> (s=itemLhs it) /\ (q++r = itemFstRhs it ++ itemSndRhs it)``,
+ ``∀it.∀s q r.MEM (item s (q,r)) (ruleItems it) ⇒ (s=itemLhs it) ∧ (q++r = itemFstRhs it ++ itemSndRhs it)``,
 HO_MATCH_MP_TAC ruleItems_ind THEN SRW_TAC [] [ruleItems, itemSndRhs, itemFstRhs, itemLhs] THEN
-METIS_TAC [APPEND, APPEND_NIL, APPEND_ASSOC])
+METIS_TAC [APPEND, APPEND_NIL, APPEND_ASSOC]);
 
  val memAllItemsRules = store_thm ("memAllItemsRules",
- ``!rs s q r.MEM (item s (q,r)) (allItems rs) ==> MEM (rule s (q++r)) rs``,
+ ``∀rs s q r.MEM (item s (q,r)) (allItems rs) ⇒ MEM (rule s (q++r)) rs``,
 Induct_on `rs` THEN SRW_TAC [] [allItems] THEN
 Cases_on `h` THEN FULL_SIMP_TAC (srw_ss()) [allItems] THEN
-`(s = itemLhs (item s' ([], l))) /\ (q ++ r = itemFstRhs(item s' ([], l)) ++ itemSndRhs  (item s' ([], l)))` by METIS_TAC [itemEqRuleExists] THEN
-FULL_SIMP_TAC (srw_ss()) [itemLhs, itemFstRhs, itemSndRhs])
+IMP_RES_TAC itemEqRuleExists THEN
+FULL_SIMP_TAC (srw_ss()) [itemLhs, itemFstRhs, itemSndRhs]);
 
 
 val itemEqRuleEqAllItems = store_thm ("itemEqRuleEqAllItems",
-``!g.{x | itemEqRule g x} = (LIST_TO_SET (allItems (rules g)))``,
+``∀g.{x | itemEqRule g x} = (LIST_TO_SET (allItems (rules g)))``,
 Induct_on `rules g` THEN SRW_TAC [] [EXTENSION, EQ_IMP_THM] THEN
 Cases_on `x` THEN Cases_on `p` THEN FULL_SIMP_TAC (srw_ss()) [allItems, itemEqRule] THEN
-METIS_TAC [MEM, allItems, itemEqRule, memRuleAllItems, memAllItemsRules])
+METIS_TAC [MEM, allItems, itemEqRule, memRuleAllItems, memAllItemsRules]);
 
 
 val finite_itemEqRule = store_thm ("finite_itemEqRule",
@@ -949,47 +969,47 @@ ASSUME_TAC lemma THEN
 `{x|P x} = P` by SRW_TAC [] [EXTENSION, IN_DEF] THEN
 `itemEqRule g = {x | itemEqRule g x}` by SRW_TAC [] [EXTENSION, IN_DEF] THEN
 ONCE_ASM_REWRITE_TAC [] THEN
-METIS_TAC [itemEqRuleEqAllItems, SUBSET_FINITE, FINITE_LIST_TO_SET])
+METIS_TAC [itemEqRuleEqAllItems, SUBSET_FINITE, FINITE_LIST_TO_SET]);
 
 
 val finite_allGrItls = store_thm ("finiteAllGrItls",
-``!g.FINITE (allGrammarItls g)``,
-SRW_TAC [] [allGrammarItls, isGrammarItl, setc_flem, finite_itemEqRule])
+``∀g.FINITE (allGrammarItls g)``,
+SRW_TAC [] [allGrammarItls, isGrammarItl, setc_flem, finite_itemEqRule]);
 
 
 val prop_mem = store_thm ("prop_mem", 
-``!P l.MEM e (asNeighbours g itl l) ==> ?e'.MEM e' l /\ MEM e (asNeighbours g itl [e'])``,
+``∀P l.MEM e (asNeighbours g itl l) ⇒ ∃e'.MEM e' l ∧ MEM e (asNeighbours g itl [e'])``,
 Induct_on `l` THEN SRW_TAC [] [asNeighbours] THENL[
 METIS_TAC [asNeighbours],
 FULL_SIMP_TAC (srw_ss()) [] THEN
-Cases_on `e'`  THEN FULL_SIMP_TAC (srw_ss()) [asNeighbours] THEN METIS_TAC []])
+Cases_on `e'`  THEN FULL_SIMP_TAC (srw_ss()) [asNeighbours] THEN METIS_TAC []]);
 
 
 
 
 val validItl_evmem = store_thm ("validItl_evmem", 
-``!l.validItl g l = EVERY (itemEqRule g) l``,
+``∀l.validItl g l = EVERY (itemEqRule g) l``,
 Induct_on `l` THEN SRW_TAC [] [validItl] THEN
-Cases_on `h` THEN Cases_on `p` THEN METIS_TAC [validItl, itemEqRule])
+Cases_on `h` THEN Cases_on `p` THEN METIS_TAC [validItl, itemEqRule]);
 
 
 val validItl_symNeighbour = store_thm ("validItl_symNeighbour", 
-``!itl.validItl g itl ==> EVERY (itemEqRule g) (symNeighbour g itl sym)``,
+``∀itl.validItl g itl ⇒ EVERY (itemEqRule g) (symNeighbour g itl sym)``,
 SRW_TAC [] [symNeighbour] THEN
 `validItl g (iclosure g (moveDot itl sym))` by METIS_TAC [validItl_iclosure, validItl_md] THEN
-METIS_TAC [validItl_evmem, rmDupes_prop])
+METIS_TAC [validItl_evmem, rmDupes_prop]);
 
 
 val symNeighbour_allDistinct = store_thm ("symNeighbour_allDistinct", 
-``!g itl sym.ALL_DISTINCT (symNeighbour g itl sym)``,
-METIS_TAC [symNeighbour, alld_rmd])
+``∀g itl sym.ALL_DISTINCT (symNeighbour g itl sym)``,
+METIS_TAC [symNeighbour, alld_rmd]);
 
 
 
 val ar1 = store_thm ("ar1", 
-``!a b c.a >=c ==> (a < b + (a-c) = 0 < b-c)``,
+``∀a b c.a >=c ⇒ (a < b + (a-c) = 0 < b-c)``,
 SRW_TAC [] [EQ_IMP_THM] THEN
-DECIDE_TAC)
+DECIDE_TAC);
 
 
 
@@ -998,7 +1018,7 @@ val (visit, visit_ind) = tprove (visit_defn,
 WF_REL_TAC (`measure (\(g,sn,itl).CARD ((allGrammarItls g )DIFF (LIST_TO_SET sn)))`) THEN
 SRW_TAC [] [] THEN
 `MEM a (asNeighbours g itl (SET_TO_LIST (allSyms g)))` by METIS_TAC [diff_mem] THEN
-`?e'.MEM e' (SET_TO_LIST (allSyms g)) /\ MEM a (asNeighbours g itl [e'])` by METIS_TAC [prop_mem] THEN
+`∃e'.MEM e' (SET_TO_LIST (allSyms g)) ∧ MEM a (asNeighbours g itl [e'])` by METIS_TAC [prop_mem] THEN
 FULL_SIMP_TAC (srw_ss()) [asNeighbours] THEN
 `EVERY (itemEqRule g) a` by METIS_TAC [validItl_symNeighbour] THEN
 `ALL_DISTINCT a` by METIS_TAC [symNeighbour_allDistinct] THEN
@@ -1040,19 +1060,23 @@ SRW_TAC [] [ar1] THEN
             set sn)) INTER (allGrammarItls g)))` by METIS_TAC [mem_in, card_same_inter, FINITE_UNION, FINITE_DIFF, FINITE_LIST_TO_SET] THEN
 FULL_SIMP_TAC (arith_ss) [INTER_COMM],
 
-`CARD (allGrammarItls g) - CARD ((allGrammarItls g) INTER (LIST_TO_SET sn)) > 0` by METIS_TAC [inter_card_less, finite_allGrItls, mem_in] 
+`CARD (allGrammarItls g) - CARD ((allGrammarItls g) INTER (LIST_TO_SET sn)) > 0` 
+by METIS_TAC [inter_card_less, finite_allGrItls, mem_in] 
 THEN
-DECIDE_TAC])
+DECIDE_TAC]);
+
+val _ = save_thm ("visit",visit);
+val _ = save_thm ("visit_ind",visit_ind);
 
 
 val slrML4Sym = Define `
-(slrML4Sym g [] sym = SOME (sgoto g, reduce g)) /\
+(slrML4Sym g [] sym = SOME (sgoto g, reduce g)) ∧
 (slrML4Sym g (i::itl) sym = 
 let
 s = sgoto g i sym 
 in
 let
-r = reduce g i (sym2Str sym)
+r = reduce g i (ts2str sym)
 in
 case (s,r) of 
                      ([],[]) -> slrML4Sym g itl sym
@@ -1060,48 +1084,51 @@ case (s,r) of
                     || ([],v12::v16::v17) -> NONE
                     || (v8::v9,[]) -> slrML4Sym g itl sym
                     || (v8::v9,[v20]) -> NONE
-                    || (v8::v9,v20::v26::v27) -> NONE)`
+                    || (v8::v9,v20::v26::v27) -> NONE)`;
 
 
 val slrML = Define `
-(slrML g itl [] = SOME (sgoto g, reduce g)) /\
+(slrML g itl [] = SOME (sgoto g, reduce g)) ∧
 (slrML g itl (sym::rst) = 
-if (slrML4Sym g itl sym = NONE) then NONE else slrML g itl rst)` 
+if (slrML4Sym g itl sym = NONE) then NONE else slrML g itl rst)`;
 
 
 
-val findItemInRules = Define `(findItemInRules (item l1 (r1,[])) [] = F) /\
-(findItemInRules (item l1 (r1,[])) ((rule l2 r2)::rst) = T) /\
-(findItemInRules (item l1 (r1,[])) (_::rst) = findItemInRules (item l1 (r1,[])) rst) /\
-(findItemInRules _ _ = F)`
+val findItemInRules = Define 
+`(findItemInRules (item l1 (r1,[])) [] = F) ∧
+(findItemInRules (item l1 (r1,[])) ((rule l2 r2)::rst) = T) ∧
+(findItemInRules (item l1 (r1,[])) (_::rst) = 
+ findItemInRules (item l1 (r1,[])) rst) ∧
+(findItemInRules _ _ = F)`;
 
 val itemEqRuleList_defn = Hol_defn "itemEqRuleList_defn"
-`(itemEqRuleList [] [] = T) /\
-(itemEqRuleList [] _ = T) /\
-(itemEqRuleList _ [] = F) /\
-(itemEqRuleList l1 l2 = if ~(LENGTH l1 = LENGTH l2) then F
-		     else
-			   if (findItemInRules (HD l1) l2) then itemEqRuleList (TL l1) l2
-			   else F)`
+`(itemEqRuleList [] [] = T) ∧
+(itemEqRuleList [] _ = T) ∧
+(itemEqRuleList _ [] = F) ∧
+(itemEqRuleList l1 l2 = 
+ if ~(LENGTH l1 = LENGTH l2) then F
+ else
+     if (findItemInRules (HD l1) l2) then itemEqRuleList (TL l1) l2
+     else F)`;
 
 
 val (itemEqRuleList,itemEqRuleList_ind) = tprove (itemEqRuleList_defn,
 WF_REL_TAC (`measure (\(l1,l2).LENGTH l1)`) THEN	
-SRW_TAC [] [])
+SRW_TAC [] []);
 
 		
-
-val getState = Define `(getState (sg,red) (itl:item list) sym = 
+val getState = Define 
+`(getState (sg,red) (itl:('nts,'ts)item list) (sym:('nts,'ts) symbol) = 
              let 
                 newitl = sg itl sym and
-                rl =  (red itl (sym2Str sym))
+                rl =  (red itl (ts2str sym))
 	     in
 			case (newitl,rl) of ([],[]) -> NA 
 			|| ([],(y::ys)) -> if (LENGTH rl = 1) then REDUCE  (HD rl) 
 					   else NA 
 			|| ((x::xs),[]) -> GOTO newitl
 			|| ((x::xs),(y::ys)) -> if (itemEqRuleList (x::xs) (y::ys))
-						    then REDUCE (HD rl) else NA)`
+						    then REDUCE (HD rl) else NA)`;
 
 
 
@@ -1116,34 +1143,34 @@ val getState = Define `(getState (sg,red) (itl:item list) sym =
 (* parse :: machine -> (symbol list, (state,ptree) list) -> (symbol list, (state, ptree) list) option *)
 
 val md_append = store_thm ("md_append", 
-``!l1 l2.moveDot (l1++l2) sym = moveDot l1 sym ++ moveDot l2 sym``,
+``∀l1 l2.moveDot (l1++l2) sym = moveDot l1 sym ++ moveDot l2 sym``,
 Induct_on `l1` THEN Induct_on `l2` THEN SRW_TAC [] [moveDot] THEN
 Cases_on `h'` THEN Cases_on `p` THEN Cases_on `r` THEN Cases_on `h'=sym` THEN
-FULL_SIMP_TAC (srw_ss()) [moveDot])
+FULL_SIMP_TAC (srw_ss()) [moveDot]);
 
 
 val iclosure_mem = store_thm ("iclosure_mem",
-``!g l.MEM e l ==> MEM e (iclosure g l)``,
+``∀g l.MEM e l ⇒ MEM e (iclosure g l)``,
 HO_MATCH_MP_TAC iclosure_ind THEN SRW_TAC [] [iclosure, LET_THM] THEN
-METIS_TAC [rmd_r2, iclosure1_mem, MEM])
+METIS_TAC [rmd_r2, iclosure1_mem, MEM]);
 
 val sgoto_mem = store_thm ("sgoto_mem", 
-``MEM (item s (q,sym::t)) itl ==> (MEM (item s (q++[sym],t)) (sgoto ag itl sym))``,
+``MEM (item s (q,sym::t)) itl ⇒ (MEM (item s (q++[sym],t)) (sgoto ag itl sym))``,
 SRW_TAC [] [sgoto, nextState] THEN
 FULL_SIMP_TAC (srw_ss()) [rgr_r9eq, md_append, moveDot] THEN
-METIS_TAC [rgr_r9eq, iclosure_mem])
+METIS_TAC [rgr_r9eq, iclosure_mem]);
 
 val reduce_append = store_thm ("reduce_append",
 ``reduce g (l1++l2) sym = reduce g l1 sym ++ reduce g l2 sym``,
 Induct_on `l1` THEN Induct_on `l2` THEN SRW_TAC [] [reduce] THEN
 Cases_on `h'` THEN Cases_on `p` THEN Cases_on `r` THEN
-METIS_TAC [APPEND, CONS, reduce])
+METIS_TAC [APPEND, CONS, reduce]);
 
 
 
 
 val trans_snoc = store_thm("trans_snoc",
-  ``!s. 
+  ``∀s. 
       trans ag (s, vp ++ [h]) =
         case trans ag (s, vp) of 
            NONE -> NONE
@@ -1154,47 +1181,48 @@ val trans_snoc = store_thm("trans_snoc",
 
 
 val initProds2Items_append = store_thm ("initProds2Items_append",
-``!r1 r2.(initProds2Items s (r1 ++ r2) = 
+``∀r1 r2.(initProds2Items s (r1 ++ r2) = 
  initProds2Items s r1 ++ initProds2Items s r2)``,
 Induct_on `r1` THEN Induct_on `r2` THEN
 SRW_TAC [] [initProds2Items] THEN
 Cases_on `h'` THEN SRW_TAC [] [initProds2Items] THEN
-METIS_TAC [])
+METIS_TAC []);
  
 val memInitProds = store_thm ("memInitProds",
-``MEM (rule (startSym ag) rhs) (rules ag) ==> 
+``MEM (rule (startSym ag) rhs) (rules ag) ⇒ 
     MEM (item (startSym ag) ([],rhs)) (initItems ag (rules ag))``,
 SRW_TAC [] [initItems, rgr_r9eq] THEN
 SRW_TAC [] [initProds2Items_append, initProds2Items] THEN
-METIS_TAC [iclosure_mem, MEM, MEM_APPEND, rgr_r9eq])
+METIS_TAC [iclosure_mem, MEM, MEM_APPEND, rgr_r9eq]);
 
 
 val sublemma = store_thm("sublemma",
-  ``!pfx sfx. 
-      NRC (rderives g) n [NTS st] (pfx ++ [NTS nt] ++ sfx) /\ 
-      0 < n ==>
-      ?m1 m2 pfx1 pfx2 sfx1 sfx2 sfx2' nt'. 
-          m1 < n /\ m2 < n /\
+  ``∀pfx sfx. 
+      NRC (rderives g) n [NTS st] (pfx ++ [NTS nt] ++ sfx) ∧ 
+      0 < n ⇒
+      ∃m1 m2 pfx1 pfx2 sfx1 sfx2 sfx2' nt'. 
+          m1 < n ∧ m2 < n ∧
           NRC (rderives g) m1 [NTS st] 
-              (pfx1 ++ [NTS nt'] ++ sfx1) /\
-          MEM (rule nt' (pfx2 ++ [NTS nt] ++ sfx2)) (rules g) /\
-          EVERY isTmnlSym sfx1 /\
+              (pfx1 ++ [NTS nt'] ++ sfx1) ∧
+          MEM (rule nt' (pfx2 ++ [NTS nt] ++ sfx2)) (rules g) ∧
+          EVERY isTmnlSym sfx1 ∧
           NRC (rderives g) m2 
               (pfx1 ++ pfx2 ++ [NTS nt] ++ sfx2 ++ sfx1) 
-              (pfx1 ++ pfx2 ++ [NTS nt] ++ sfx2' ++ sfx1) /\
-          (pfx = pfx1 ++ pfx2) /\ (sfx = sfx2' ++ sfx1)``,
+              (pfx1 ++ pfx2 ++ [NTS nt] ++ sfx2' ++ sfx1) ∧
+          (pfx = pfx1 ++ pfx2) ∧ (sfx = sfx2' ++ sfx1)``,
+
   Induct_on `n` THEN SRW_TAC [][NRC_SUC_RECURSE_LEFT] THEN
   Cases_on `0<n` THENL[
-    `?pfx0 sfx0 Nt1 rhs.
-        (z=pfx0++[NTS Nt1]++sfx0) /\
-        (pfx++[NTS nt]++sfx = pfx0++rhs++sfx0) /\
-        MEM (rule Nt1 rhs) (rules g) /\
+    `∃pfx0 sfx0 Nt1 rhs.
+        (z=pfx0++[NTS Nt1]++sfx0) ∧
+        (pfx++[NTS nt]++sfx = pfx0++rhs++sfx0) ∧
+        MEM (rule Nt1 rhs) (rules g) ∧
         EVERY isTmnlSym sfx0` 
       by METIS_TAC [rderives_def] THEN
     SRW_TAC [] [] THEN
     Cases_on `IS_PREFIX pfx0 pfx` THENL[
-      Cases_on `pfx0=pfx` THENL[
-        SRW_TAC [] [] THEN
+      Cases_on `pfx0=pfx` THEN1
+        (SRW_TAC [] [] THEN
         Cases_on `rhs` THEN
         SRW_TAC [] [] THEN
         FULL_SIMP_TAC (srw_ss()) [] THENL[
@@ -1210,14 +1238,14 @@ val sublemma = store_thm("sublemma",
           MAP_EVERY Q.EXISTS_TAC [`n`, `0`, `pfx`, `[]`, 
                                   `sfx0`, `t`, `t`, `Nt1`] THEN 
           SRW_TAC [][]
-        ],
+        ]) THEN
 
         (* pfx \neq pfx0 *)
-        `?t. pfx0 = pfx ++ NTS nt :: t`
-           by (`?l. pfx0 = pfx ++ l` 
+        `∃t. pfx0 = pfx ++ NTS nt :: t`
+           by (`∃l. pfx0 = pfx ++ l` 
                  by METIS_TAC [IS_PREFIX_APPEND] THEN 
                SRW_TAC [][] THEN 
-               `?hl tl. l = hl :: tl`
+               `∃hl tl. l = hl :: tl`
                   by (Cases_on `l` THEN 
                       FULL_SIMP_TAC (srw_ss()) []) THEN 
                SRW_TAC [][] THEN 
@@ -1227,31 +1255,35 @@ val sublemma = store_thm("sublemma",
         `NRC (rderives g) n [NTS st]
              (pfx ++ [NTS nt] ++ (t ++ [NTS Nt1] ++ sfx0))`
            by METIS_TAC [APPEND_ASSOC, APPEND] THEN 
-        `?m1 m2 p1 p2 s1 s2 s2' nt'.
-            m1 < n /\ m2 < n /\ 
-            NRC (rderives g) m1 [NTS st] (p1 ++ [NTS nt'] ++ s1) /\
-            MEM (rule nt' (p2 ++ [NTS nt] ++ s2)) (rules g) /\
-            EVERY isTmnlSym s1 /\
+        `∃m1 m2 p1 p2 s1 s2 s2' nt'.
+            m1 < n ∧ m2 < n ∧ 
+            NRC (rderives g) m1 [NTS st] (p1 ++ [NTS nt'] ++ s1) ∧
+            MEM (rule nt' (p2 ++ [NTS nt] ++ s2)) (rules g) ∧
+            EVERY isTmnlSym s1 ∧
             NRC (rderives g) m2 
                 (p1 ++ p2 ++ [NTS nt] ++ s2 ++ s1)
-                (p1 ++ p2 ++ [NTS nt] ++ s2' ++ s1) /\
-            (pfx = p1 ++ p2) /\ 
+                (p1 ++ p2 ++ [NTS nt] ++ s2' ++ s1) ∧
+            (pfx = p1 ++ p2) ∧ 
             (t ++ [NTS Nt1] ++ sfx0 = s2' ++ s1)`
            by METIS_TAC [] THEN 
         `isSuffix s1 sfx0`
-           by (`isSuffix s1 sfx0 \/ isSuffix sfx0 s1`
+           by (`isSuffix s1 sfx0 ∨ isSuffix sfx0 s1`
                  by METIS_TAC [append_eq_imp_sfx, APPEND_ASSOC] THEN
-               `?foo. s1 = foo ++ sfx0` 
+               `∃foo. s1 = foo ++ sfx0` 
                  by METIS_TAC [isSuffix_APPEND] THEN 
                Cases_on `foo` THEN SRW_TAC [][] THEN 
                `s2' ++ h::t' = t ++ [NTS Nt1]`
                   by METIS_TAC [APPEND_11, APPEND_ASSOC] THEN
-               `LAST (h::t') = NTS Nt1` by METIS_TAC [NOT_CONS_NIL, last_elem, last_append] THEN
+               `LAST (h::t') = NTS Nt1` by METIS_TAC [NOT_CONS_NIL, last_elem, 
+						      last_append] THEN
                `MEM (LAST (h::t')) (h::t')`
                  by METIS_TAC [MEM_APPEND, APPEND_FRONT_LAST, 
                                MEM] THEN 
-               METIS_TAC [isTmnlSymML, EVERY_MEM, EVERY_APPEND]) THEN
-        `?sf1. sfx0 = sf1 ++ s1` by METIS_TAC [isSuffix_APPEND] THEN 
+		 `isWord [NTS Nt1]` by 
+		 METIS_TAC [APPEND_FRONT_LAST, NOT_CONS_NIL, EVERY_MEM, 
+			    EVERY_APPEND] THEN
+		 FULL_SIMP_TAC (srw_ss()) [isTmnlSym_def]) THEN
+        `∃sf1. sfx0 = sf1 ++ s1` by METIS_TAC [isSuffix_APPEND] THEN 
         SRW_TAC [][] THEN 
         MAP_EVERY Q.EXISTS_TAC [`m1`, `SUC m2`, 
                                 `p1`, `p2`, `s1`, `s2`, 
@@ -1265,17 +1297,16 @@ val sublemma = store_thm("sublemma",
 
           FULL_SIMP_TAC bool_ss [GSYM APPEND_ASSOC, APPEND_11, 
                                  APPEND, CONS_11]
-        ]
-      ],
+        ],
 
       
-      `IS_PREFIX pfx pfx0 \/ IS_PREFIX pfx0 pfx`
+      `IS_PREFIX pfx pfx0 ∨ IS_PREFIX pfx0 pfx`
 	  by METIS_TAC [append_eq_imp_pfx, APPEND_ASSOC] THEN
       FULL_SIMP_TAC (srw_ss()) [IS_PREFIX_APPEND] THEN
       SRW_TAC [] [] THEN
       `l++[NTS nt]++sfx = rhs++sfx0` 
 	  by METIS_TAC [APPEND_11, APPEND_ASSOC] THEN
-      Q_TAC SUFF_TAC `?sf1.(sfx = sf1 ++ sfx0)`
+      Q_TAC SUFF_TAC `∃sf1.(sfx = sf1 ++ sfx0)`
       THENL[
 	    SRW_TAC [] [] THEN
 	    `rhs=l++[NTS nt]++sf1` 
@@ -1287,10 +1318,10 @@ val sublemma = store_thm("sublemma",
                                 `Nt1`] THEN 
             SRW_TAC [ARITH_ss][],
 	    
-	`(l=rhs) \/
-         (?p s.(rhs=l++[NTS nt]++p) 
-          /\ (sfx=p++s)) \/
-         (?p s.(l=p++s) /\
+	`(l=rhs) ∨
+         (∃p s.(rhs=l++[NTS nt]++p) 
+          ∧ (sfx=p++s)) ∨
+         (∃p s.(l=p++s) ∧
             (rhs=p))` by METIS_TAC [listCompLens] THEN
 	SRW_TAC [] []
 	 THENL[
@@ -1316,11 +1347,11 @@ val sublemma = store_thm("sublemma",
     SRW_TAC [][] THEN 
     FULL_SIMP_TAC (srw_ss()) [rderives_def, lreseq] THEN 
     METIS_TAC [APPEND_NIL]
-    ])
+    ]);
 
 
 val iclosure1_append = store_thm ("iclosure1_append",
-``!l1 l2.iclosure1 g (l1 ++ l2) = iclosure1 g l1 ++ iclosure1 g l2``,
+``∀l1 l2.iclosure1 g (l1 ++ l2) = iclosure1 g l1 ++ iclosure1 g l2``,
 Induct_on `l1` THEN Induct_on `l2` THEN SRW_TAC [] [iclosure1] THEN
 Cases_on `h'` THEN Cases_on `p` THEN Cases_on `r` 
 THENL[
@@ -1329,19 +1360,19 @@ THENL[
       Cases_on `h'` THEN SRW_TAC [] [iclosure1] THEN
       METIS_TAC [APPEND, APPEND_ASSOC, APPEND_NIL]
       ]
-)
+);
 
 
 val getItems_append = store_thm ("getItems_append",
-``!l1 l2.getItems (l1++l2) N  = getItems l1 N ++ getItems l2 N``,
+``∀l1 l2.getItems (l1++l2) N  = getItems l1 N ++ getItems l2 N``,
 Induct_on `l1` THEN Induct_on `l2` THEN SRW_TAC [] [getItems] THEN
-Cases_on `h'` THEN SRW_TAC [] [getItems])
+Cases_on `h'` THEN SRW_TAC [] [getItems]);
 
 
   
 val iclosureNtGen = store_thm ("iclosureNtGen",
-``!ag l r1.MEM (item lhs (r1,NTS N::r2)) (iclosure ag l) ==> 
- !rhs.MEM (rule N rhs) (rules ag) ==>
+``∀ag l r1.MEM (item lhs (r1,NTS N::r2)) (iclosure ag l) ⇒ 
+ ∀rhs.MEM (rule N rhs) (rules ag) ⇒
 MEM (item N ([],rhs)) (iclosure ag l)``,
 HO_MATCH_MP_TAC iclosure_ind THEN 
 SRW_TAC [] [iclosure, LET_THM] THEN
@@ -1358,13 +1389,13 @@ rmDupes (iclosure1 ag (r1''' ++ [item lhs (r1,NTS N::r2)] ++ r2'''))` by METIS_T
 FULL_SIMP_TAC (srw_ss()) [iclosure1_append, iclosure1] THEN
 `getItems (rules ag) N  = getItems (r1' ++ [rule N rhs] ++ r2') N` by METIS_TAC [] THEN
 FULL_SIMP_TAC (srw_ss()) [getItems_append, getItems] THEN
-METIS_TAC [rgr_r9eq, APPEND, rmd_r2, APPEND_ASSOC])
+METIS_TAC [rgr_r9eq, APPEND, rmd_r2, APPEND_ASSOC]);
 
 val transOutMem = store_thm("transOutMem",
-``!g s s0 vp1 nt sfx nt'.
-  (trans g (iclosure g s0,vp1) = SOME s) ==>
-  MEM (item nt' (r1,NTS nt::sfx)) s ==>
-  MEM (rule nt rhs) (rules g) ==>
+``∀g s s0 vp1 nt sfx nt'.
+  (trans g (iclosure g s0,vp1) = SOME s) ⇒
+  MEM (item nt' (r1,NTS nt::sfx)) s ⇒
+  MEM (rule nt rhs) (rules g) ⇒
   MEM (item nt ([],rhs)) s``,
 Induct_on `vp1` THEN SRW_TAC [] []THEN
 FULL_SIMP_TAC (srw_ss()) [trans] THEN
@@ -1376,12 +1407,12 @@ THENL[
       FULL_SIMP_TAC (srw_ss()) [] THEN
       SRW_TAC [] [] THEN
       METIS_TAC []
-      ])
+      ]);
 
 
 val transExists = store_thm ("transExists",
-``! nt r1 vp rst s.MEM (item nt (r1,vp++rst)) s ==>
-  ?s'.(trans g (s, vp) = SOME s') /\ 
+``∀ nt r1 vp rst s.MEM (item nt (r1,vp++rst)) s ⇒
+  ∃s'.(trans g (s, vp) = SOME s') ∧ 
        MEM (item nt (r1++vp, rst)) s'``,
 Induct_on `vp` THEN SRW_TAC [] [trans] THEN
 `~(moveDot s h = [])` by (FULL_SIMP_TAC (srw_ss()) [rgr_r9eq, md_append, moveDot] THEN
@@ -1397,48 +1428,48 @@ FULL_SIMP_TAC (srw_ss()) [rgr_r9eq] THEN
 SRW_TAC [] []THEN
 FULL_SIMP_TAC (srw_ss()) [md_append, moveDot] THEN
 METIS_TAC [MEM, MEM_APPEND, rgr_r9eq]) THEN
-METIS_TAC [c1, iclosure_mem])
+METIS_TAC [c1, iclosure_mem]);
       
 
 val transSeq = store_thm ("transSeq",
-``!s s' vp sp' s''.
-  (trans g (iclosure g s, vp) = SOME s') ==>
-  (trans g (s',vp') = SOME s'') ==>
+``∀s s' vp sp' s''.
+  (trans g (iclosure g s, vp) = SOME s') ⇒
+  (trans g (s',vp') = SOME s'') ⇒
   (trans g (iclosure g s, vp++vp') = SOME s'')``,
 Induct_on `vp` THEN SRW_TAC [] [trans] THEN
 Cases_on `moveDot (iclosure g s) h` THEN
 SRW_TAC [] [] THEN
 FULL_SIMP_TAC (srw_ss()) []
-)
+);
 
 
 val ic1Delete = store_thm 
 ("ic1Delete",
-``!e h l.~(e=h) ==> ~(MEM e l) ==>
-   MEM e (iclosure1 g l) ==> 
-   MEM e (iclosure1 g [h]) \/ (MEM e (iclosure1 g (delete h l)))``,
+``∀e h l.~(e=h) ⇒ ~(MEM e l) ⇒
+   MEM e (iclosure1 g l) ⇒ 
+   MEM e (iclosure1 g [h]) ∨ (MEM e (iclosure1 g (delete h l)))``,
 Induct_on `l` THEN SRW_TAC [] [delete_def,iclosure1] THEN
 `(iclosure1 g (h::l) = iclosure1 g [h] ++ iclosure1 g l)`
     by METIS_TAC [iclosure1_append,APPEND] THEN
 FULL_SIMP_TAC (srw_ss()) [] THEN
-METIS_TAC [iclosure1_append,APPEND,MEM_APPEND])
+METIS_TAC [iclosure1_append,APPEND,MEM_APPEND]);
 
 
 val ic1Delete2 = store_thm 
 ("ic1Delete2",
-``!e h l.~(e=h) ==> ~(MEM e (delete h l)) ==>
-   MEM e (iclosure1 g (delete h l)) ==> 
-   MEM e (iclosure1 g [h]) \/ (MEM e (iclosure1 g l))``,
+``∀e h l.~(e=h) ⇒ ~(MEM e (delete h l)) ⇒
+   MEM e (iclosure1 g (delete h l)) ⇒ 
+   MEM e (iclosure1 g [h]) ∨ (MEM e (iclosure1 g l))``,
 Induct_on `l` THEN SRW_TAC [] [delete_def,iclosure1] THEN
 `(iclosure1 g (h::l) = iclosure1 g [h] ++ iclosure1 g l)`
     by METIS_TAC [iclosure1_append,APPEND] THEN
 FULL_SIMP_TAC (srw_ss()) [] THEN
-METIS_TAC [iclosure1_append,APPEND,MEM_APPEND])
+METIS_TAC [iclosure1_append,APPEND,MEM_APPEND]);
 
 
 val iclosure1RmdMem =
 store_thm ("iclosure1RmdMem",
-``!e l.MEM e (iclosure1 g l) = MEM e (iclosure1 g (rmDupes l))``,
+``∀e l.MEM e (iclosure1 g l) = MEM e (iclosure1 g (rmDupes l))``,
 
 Induct_on `l` THEN SRW_TAC [] [iclosure1,rmDupes,EQ_IMP_THM] THEN
 `(iclosure1 g (h::l) = iclosure1 g [h] ++ iclosure1 g l)`
@@ -1474,11 +1505,11 @@ THENL[
 		by METIS_TAC [rmd_mem_list,delete_mem_list] THEN
 	    `~MEM e (rmDupes (delete h l))` by
 	    METIS_TAC [rmd_mem_list,delete_mem_list] THEN
-	    `!e h l.
-            ~(e = h) ==>
-            ~MEM e l ==>
-            MEM e (iclosure1 g l) ==>
-            MEM e (iclosure1 g [h]) \/ MEM e (iclosure1 g (delete h l))`
+	    `∀e h l.
+            ~(e = h) ⇒
+            ~MEM e l ⇒
+            MEM e (iclosure1 g l) ⇒
+            MEM e (iclosure1 g [h]) ∨ MEM e (iclosure1 g (delete h l))`
 		by METIS_TAC [ic1Delete] THEN
 	    FIRST_X_ASSUM (Q.SPECL_THEN [`e`,`h`,`rmDupes (delete h l)`] MP_TAC) THEN
 	    SRW_TAC [][] THEN
@@ -1490,79 +1521,75 @@ THENL[
 	    FULL_SIMP_TAC (srw_ss()) [] THEN
 	    METIS_TAC [rmd_mem_list,iclosure1_mem,delete_mem_list,ic1Delete2]
 	    ]
-      ])
+      ]);
 
 
 val ic1ImpIcMem =
 store_thm ("ic1ImpIcMem",
-``!e l.MEM e (iclosure1 g l) ==> MEM e (iclosure g l)``,
+``∀e l.MEM e (iclosure1 g l) ⇒ MEM e (iclosure g l)``,
 Induct_on `l` THEN SRW_TAC [] [iclosure,iclosure1,LET_THM] THEN
-METIS_TAC [iclosure1RmdMem,rmd_mem_list,iclosure_mem])
+METIS_TAC [iclosure1RmdMem,rmd_mem_list,iclosure_mem]);
 
 
 val icImpIcTwice =
 store_thm ("icImpIcTwice",
-``!g l.MEM e (iclosure g l) ==> MEM e (iclosure g (iclosure g l))``,
+``∀g l.MEM e (iclosure g l) ⇒ MEM e (iclosure g (iclosure g l))``,
 HO_MATCH_MP_TAC iclosure_ind THEN
 SRW_TAC [][iclosure,LET_THM] THEN
-METIS_TAC [iclosure_mem])
+METIS_TAC [iclosure_mem]);
 
 val icEqIc1 = store_thm
 ("icEqIc1",
-``!g l.(set (rmDupes l) = set (rmDupes (iclosure1 g (rmDupes l)))) ==>
+``∀g l.(set (rmDupes l) = set (rmDupes (iclosure1 g (rmDupes l)))) ⇒
   (rmDupes (iclosure1 g (rmDupes l)) = iclosure g l)``,
 HO_MATCH_MP_TAC iclosure_ind THEN
 SRW_TAC [] [iclosure,iclosure1] THEN
-FULL_SIMP_TAC (srw_ss()) [rmDupes,iclosure1,LET_THM])
+FULL_SIMP_TAC (srw_ss()) [rmDupes,iclosure1,LET_THM]);
 
 val _ = Globals.linewidth := 60
 
 val forallItem = store_thm ("forallItem",
-``(!h.P h) = !N l1 l2.P (item N (l1,l2))``,
+``(∀h.P h) = ∀N l1 l2.P (item N (l1,l2))``,
 SRW_TAC [][EQ_IMP_THM] THEN
 Cases_on `h` THEN
-Cases_on `p` THEN SRW_TAC [][])
+Cases_on `p` THEN SRW_TAC [][]);
 
 val forallRule = store_thm ("forallRule",
-``(!h.P h) = !N rhs.P (rule N rhs)``,
+``(∀h.P h) = ∀N rhs.P (rule N rhs)``,
 SRW_TAC [][EQ_IMP_THM] THEN
 Cases_on `h` THEN
-SRW_TAC [][])
+SRW_TAC [][]);
 
 
 
 val getItemsInRule = 
 store_thm ("getItemsInRule",
-``!l N l1 l2 nt.MEM (item N (l1,l2)) (getItems l nt) =
-  (N=nt) /\ MEM (rule N (l1++l2)) l /\ (l1=[])``,
+``∀l N l1 l2 nt.MEM (item N (l1,l2)) (getItems l nt) =
+  (N=nt) ∧ MEM (rule N (l1++l2)) l ∧ (l1=[])``,
 Induct_on `l` THEN 
 ASM_SIMP_TAC (srw_ss()) [forallRule,getItems] THEN
 SRW_TAC [][] THEN
-METIS_TAC [APPEND_NIL])
+METIS_TAC [APPEND_NIL]);
 
 
 val iclosure1MemType = store_thm
 ("iclosure1MemType",
-``!e l.MEM e (iclosure1 g l) =
-  MEM e l \/ 
-?N M p s r.MEM (rule N r) (rules g) /\
-(MEM (item M (p,NTS N::s)) l) /\
+``∀e l.MEM e (iclosure1 g l) =
+  MEM e l ∨ 
+∃N M p s r.MEM (rule N r) (rules g) ∧
+(MEM (item M (p,NTS N::s)) l) ∧
  (e=item N ([],r)) ``,
+
 Induct_on `l` THEN 
 ASM_SIMP_TAC (srw_ss()) [iclosure1,forallItem] THEN
 SRW_TAC [][] THEN
-Cases_on `l2` THEN SRW_TAC [] [iclosure1] 
-THENL[
-      METIS_TAC [],
+Cases_on `l2` THEN SRW_TAC [] [iclosure1] THEN1
+ METIS_TAC [] THEN
 
-      Cases_on `h` THEN SRW_TAC [] [iclosure1] 
-      THENL[
-	    METIS_TAC [],
+ Cases_on `h` THEN SRW_TAC [] [iclosure1] THEN
+ SRW_TAC [] [getItemsInRule] THEN
+ METIS_TAC [APPEND_NIL]);
 
-	    SRW_TAC [] [getItemsInRule] THEN
-	    METIS_TAC [APPEND_NIL]	    
-	    ]
-      ])
 
 val iclosure' = prove(
   ``iclosure g l = 
@@ -1576,22 +1603,22 @@ val iclosure_NIL = store_thm(
   "iclosure_NIL",
   ``iclosure g [] = []``,
   SRW_TAC [][iclosure]);
-val _ =export_rewrites ["iclosure_NIL"]
+val _ =export_rewrites ["iclosure_NIL"];
 
 val set_rmDupes = store_thm(
   "set_rmDupes",
   ``set (rmDupes l) = set l``,
-  MATCH_ACCEPT_TAC (GSYM rmDupes_lts))
-val _ = export_rewrites ["set_rmDupes"]
+  MATCH_ACCEPT_TAC (GSYM rmDupes_lts));
+val _ = export_rewrites ["set_rmDupes"];
   
 
 val iclosure_ind' = prove(
-  ``!P. (!g l. (!ril al. (ril = rmDupes l) /\
-                         (al = rmDupes (iclosure1 g ril)) /\
-                         ~(set ril = set al) ==> 
-                         P g al) ==>
-               P g l) ==>
-        !v v1. P v v1``,
+  ``∀P. (∀g l. (∀ril al. (ril = rmDupes l) ∧
+                         (al = rmDupes (iclosure1 g ril)) ∧
+                         ~(set ril = set al) ⇒ 
+                         P g al) ⇒
+               P g l) ⇒
+        ∀v v1. P v v1``,
   NTAC 2 STRIP_TAC THEN 
   HO_MATCH_MP_TAC iclosure_ind THEN SRW_TAC [][] THEN 
   FIRST_X_ASSUM MATCH_MP_TAC THEN 
@@ -1600,27 +1627,27 @@ val iclosure_ind' = prove(
 
 val ic1EqSet = store_thm
 ("ic1EqSet",
-``!l l'.(set l = set l') ==>
+``∀l l'.(set l = set l') ⇒
 ((set (iclosure1 g l)) = set (iclosure1 g l'))``,
 SRW_TAC [][ EXTENSION,EQ_IMP_THM] THEN
 FULL_SIMP_TAC (srw_ss()) [iclosure1MemType] THEN
-METIS_TAC [])
+METIS_TAC []);
 
 val ic1EqSetRmd = store_thm
 ("ic1EqSetRmd",
-``!l l'.(set l = set l') ==>
+``∀l l'.(set l = set l') ⇒
 ((set (iclosure1 g l)) = set (iclosure1 g (rmDupes l')))``,
 SRW_TAC [] [] THEN
 SRW_TAC [][ EXTENSION,EQ_IMP_THM] THEN
 `((set (iclosure1 g l)) = set (iclosure1 g l'))`
     by METIS_TAC [ic1EqSet] THEN
 FULL_SIMP_TAC (srw_ss()) [EXTENSION] THEN
-METIS_TAC [iclosure1RmdMem])
+METIS_TAC [iclosure1RmdMem]);
 
 
 val icTwiceImpIc =
 store_thm ("icTwiceImpIc",
-``!g l.MEM e (iclosure g (iclosure g l)) ==> 
+``∀g l.MEM e (iclosure g (iclosure g l)) ⇒ 
 	  MEM e (iclosure g l)``,
 HO_MATCH_MP_TAC iclosure_ind' THEN
 REPEAT GEN_TAC THEN STRIP_TAC THEN 
@@ -1646,19 +1673,19 @@ THENL[
       FULL_SIMP_TAC (srw_ss()) [] THEN
       Q.ABBREV_TAC `l'=(iclosure1 g (rmDupes l))` THEN
       METIS_TAC [ic1EqSet,mem_in,iclosure1RmdMem,rmd_mem_list]
-      ])
+      ]);
 
 val iclosureTwice =
 store_thm ("iclosureTwice",
-``!g l.set (iclosure g (iclosure g l)) = set (iclosure g l)``,
+``∀g l.set (iclosure g (iclosure g l)) = set (iclosure g l)``,
 SRW_TAC [] [EXTENSION,EQ_IMP_THM] THEN
- METIS_TAC [icTwiceImpIc,icImpIcTwice])
+ METIS_TAC [icTwiceImpIc,icImpIcTwice]);
 
 
 val mdMem = store_thm ("mdMem",
-``!e itl sym.MEM e (moveDot itl sym) ==>  
-?l r1 r2.(e=item l (r1++[sym],r2)) 
-/\ (MEM (item l (r1,sym::r2)) itl)``,
+``∀e itl sym.MEM e (moveDot itl sym) ⇒  
+∃l r1 r2.(e=item l (r1++[sym],r2)) 
+∧ (MEM (item l (r1,sym::r2)) itl)``,
 Induct_on `itl` THEN SRW_TAC [] [moveDot] THEN
 `moveDot (h::itl) sym = 
 moveDot [h] sym ++ moveDot itl sym` by METIS_TAC [md_append, APPEND] THEN
@@ -1667,19 +1694,19 @@ THENL[
       Cases_on `h` THEN Cases_on `p` THEN Cases_on `r` THEN
       FULL_SIMP_TAC (srw_ss()) [moveDot] THEN
       Cases_on `h=sym` THEN FULL_SIMP_TAC (srw_ss()) [],
-      METIS_TAC []])
+      METIS_TAC []]);
 
 
 val mdMemExists = store_thm ("mdMemExists",
-``!itl r1 r2 h.MEM (item lhs (r1,h::r2)) itl ==>
+``∀itl r1 r2 h.MEM (item lhs (r1,h::r2)) itl ⇒
   MEM (item lhs (r1++[h],r2)) (moveDot itl h)``,
 SRW_TAC [][rgr_r9eq,md_append]  THEN
 SRW_TAC [] [md_append,moveDot] THEN
-METIS_TAC [APPEND_NIL])
+METIS_TAC [APPEND_NIL]);
 
 val mdSetEq = store_thm
 ("mdSetEq",
-``!l l' h.(set l = set l') ==>
+``∀l l' h.(set l = set l') ⇒
   (set (moveDot l h) = set (moveDot l' h))``,
 Induct_on `l` THEN SRW_TAC [][moveDot,EQ_IMP_THM,EXTENSION] THEN
 FULL_SIMP_TAC (srw_ss()) []
@@ -1695,15 +1722,14 @@ THENL[
       IMP_RES_TAC mdMem THEN
       SRW_TAC [][] THEN
       METIS_TAC [mdMem,mdMemExists,MEM]
-      ])
+      ]);
       
-fun MAGIC (asl, w) = ACCEPT_TAC (mk_thm(asl,w)) (asl,w) 
 
 val iclosureMemIc1 = store_thm
 ("iclosureMemIc1",
-``!g l.MEM e (iclosure g l) =
-  MEM e l \/ ?e'.MEM e' l /\ MEM e (iclosure g [e'])``,
-MAGIC)
+``∀g l.MEM e (iclosure g l) =
+  MEM e l ∨ ∃e'.MEM e' l ∧ MEM e (iclosure g [e'])``,
+MAGIC);
 (*
 HO_MATCH_MP_TAC iclosure_ind' THEN
 
@@ -1736,7 +1762,7 @@ THENL[
 		  Q.EXISTS_TAC `item M (p,NTS N::s)` THEN
 		  SRW_TAC [][] THEN
 		  SRW_TAC [] [rmDupes,delete_def,iclosure1,getItems,getItems_append] THEN
-		  `?r1 r2.rules g = r1++[rule N r]++r2`
+		  `∃r1 r2.rules g = r1++[rule N r]++r2`
 		      by METIS_TAC [rgr_r9eq] THEN
 		  SRW_TAC [][getItems_append,getItems] THEN
 		  METIS_TAC [iclosure_mem,rmd_mem_list,MEM,MEM_APPEND],
@@ -1752,7 +1778,7 @@ THENL[
 			Q.EXISTS_TAC `item M (p,NTS N::s)` THEN
 			SRW_TAC [][] THEN
 			FULL_SIMP_TAC (srw_ss()) [rmDupes,delete_def,iclosure1] THEN
-			`?r1 r2.rules g = r1++[rule N r]++r2`
+			`∃r1 r2.rules g = r1++[rule N r]++r2`
 			    by METIS_TAC [rgr_r9eq] THEN
 			SRW_TAC [][getItems_append,getItems] THEN
 			MAGIC,
@@ -1768,7 +1794,7 @@ THENL[
       Q.EXISTS_TAC `item M (p,NTS N::s)` THEN
       SRW_TAC [][] THEN
       SRW_TAC [] [rmDupes,delete_def,iclosure1,getItems,getItems_append] THEN
-      `?r1 r2.rules g = r1++[rule N r]++r2`
+      `∃r1 r2.rules g = r1++[rule N r]++r2`
 	  by METIS_TAC [rgr_r9eq] THEN
       SRW_TAC [][getItems_append,getItems] THEN
       METIS_TAC [iclosure_mem,rmd_mem_list,MEM,MEM_APPEND]
@@ -1779,15 +1805,15 @@ THENL[
 val iclosure_APPEND = 
 store_thm ("iclosure_APPEND",
 ``MEM e (iclosure g (l1++l2)) =
-  (MEM e (l1++l2) \/ MEM e (iclosure g l1) \/
+  (MEM e (l1++l2) ∨ MEM e (iclosure g l1) ∨
   MEM e (iclosure g l2))``,
 SRW_TAC [][EQ_IMP_THM] THEN
 FULL_SIMP_TAC (srw_ss()) [Once iclosureMemIc1] THEN
-METIS_TAC [iclosure_mem,iclosureMemIc1])
+METIS_TAC [iclosure_mem,iclosureMemIc1]);
 
 val iclosureSetEq = store_thm 
 ("iclosureSetEq",
-``!g l l'.(set l = set l') ==>
+``∀g l l'.(set l = set l') ⇒
   (set (iclosure g l) = set (iclosure g l'))``,
 SRW_TAC [][EXTENSION,EQ_IMP_THM,Once iclosureMemIc1]
 THENL[
@@ -1798,15 +1824,15 @@ THENL[
       METIS_TAC [iclosure_APPEND,rgr_r9eq,iclosure_mem,APPEND_ASSOC],
 
       METIS_TAC [iclosure_mem,iclosureMemIc1]
-      ])
+      ]);
 
 
 val transIcIcImpIc = store_thm (
 "transIcIcImpIc",
-``!g l l' p s.(set l = set l') ==>
-(trans g (l,p) = SOME s) ==>
-  ?s'.(trans g (l',p) = SOME s')
-/\ (set s = set s')``,
+``∀g l l' p s.(set l = set l') ⇒
+(trans g (l,p) = SOME s) ⇒
+  ∃s'.(trans g (l',p) = SOME s')
+∧ (set s = set s')``,
 Induct_on `p` THEN SRW_TAC [][]
 THENL[
       FULL_SIMP_TAC (srw_ss()) [iclosure,trans],
@@ -1824,15 +1850,15 @@ THENL[
              set (iclosure g (h''::t'))` 
 		by METIS_TAC [iclosureSetEq] THEN
 	    METIS_TAC []
-	    ]])
+	    ]]);
 
 
 val transSeqIcGen = store_thm ("transSeqIcGen",
-``!s s' vp sp' s''.
-  (trans g (iclosure g s, vp) = SOME s') ==>
-  (trans g (iclosure g s',vp') = SOME s'') ==>
-  ?s'''.(trans g (iclosure g s, vp++vp') = SOME s''')
-  /\ (set s''' = set s'')``,
+``∀s s' vp sp' s''.
+  (trans g (iclosure g s, vp) = SOME s') ⇒
+  (trans g (iclosure g s',vp') = SOME s'') ⇒
+  ∃s'''.(trans g (iclosure g s, vp++vp') = SOME s''')
+  ∧ (set s''' = set s'')``,
 Induct_on `vp` THEN SRW_TAC [] [trans] 
 THENL[
       METIS_TAC [transIcIcImpIc,iclosureTwice],
@@ -1840,21 +1866,21 @@ THENL[
       Cases_on `moveDot (iclosure g s) h` THEN
       SRW_TAC [] [] THEN
       FULL_SIMP_TAC (srw_ss()) []
-      ])
+      ]);
 
 
 val transShiftExists = store_thm ("transShiftExists",
-``!s s0 r1 vp1 vp2 nt sfx rhs.
-   (trans g (iclosure g s0,vp1) = SOME s) ==>
-    MEM (item nt' (r1,vp2++[NTS nt]++sfx)) s ==>
-    MEM (rule nt rhs) (rules g) ==>
-    ?s'.(trans g (iclosure g s0, vp1++vp2) = SOME s') /\
+``∀s s0 r1 vp1 vp2 nt sfx rhs.
+   (trans g (iclosure g s0,vp1) = SOME s) ⇒
+    MEM (item nt' (r1,vp2++[NTS nt]++sfx)) s ⇒
+    MEM (rule nt rhs) (rules g) ⇒
+    ∃s'.(trans g (iclosure g s0, vp1++vp2) = SOME s') ∧
         MEM (item nt ([],rhs)) s'``,
 Induct_on `vp2` THEN SRW_TAC [] []
 THENL[
       METIS_TAC [transOutMem],
 
-      `?s'.(trans g (iclosure g s,h::vp2) = SOME s') /\
+      `∃s'.(trans g (iclosure g s,h::vp2) = SOME s') ∧
          MEM (item nt' (r1++[h]++vp2,[NTS nt]++sfx)) s'` by 
       (SRW_TAC [] [] THEN
       SRW_TAC [] [trans] THEN
@@ -1871,7 +1897,7 @@ THENL[
                THENL[
 		     METIS_TAC [MEM, MEM_APPEND],
 
-		     `?s'.(trans g (iclosure g (h'::t),vp2) = SOME s') /\
+		     `∃s'.(trans g (iclosure g (h'::t),vp2) = SOME s') ∧
 									    MEM (item nt' (r1 ++ [h] ++ vp2,[NTS nt]++sfx)) s'` 
 			 by METIS_TAC [transExists, iclosure_mem, APPEND_ASSOC] THEN
 		     FULL_SIMP_TAC (srw_ss()) []
@@ -1880,19 +1906,19 @@ THENL[
 	    `MEM (item nt ([],rhs)) s'` by METIS_TAC [transOutMem, APPEND] THEN
 	    IMP_RES_TAC transSeqIcGen THEN
 	    METIS_TAC [mem_in]
-	    ]])
+	    ]]);
       
 
 
 val lemma =store_thm("lemma",
-  ``!n pfx sfx nt rhs. 
+  ``∀n pfx sfx nt rhs. 
       NRC (rderives ag) n [NTS (startSym ag)] 
-                          (pfx ++ [NTS nt] ++ sfx) /\
-      MEM (rule nt rhs) (rules ag) ==>
-      ?s. (trans ag (initItems ag (rules ag), pfx) = SOME s) /\
+                          (pfx ++ [NTS nt] ++ sfx) ∧
+      MEM (rule nt rhs) (rules ag) ⇒
+      ∃s. (trans ag (initItems ag (rules ag), pfx) = SOME s) ∧
           MEM (item nt ([], rhs)) s``,
   completeInduct_on `n` THEN 
-  `(n = 0) \/ ?m. n = SUC m` by METIS_TAC [num_CASES] 
+  `(n = 0) ∨ ∃m. n = SUC m` by METIS_TAC [num_CASES] 
    THENL [
 	  SRW_TAC [][] THEN 
 	  FULL_SIMP_TAC (srw_ss()) [lreseq] THEN 
@@ -1902,32 +1928,32 @@ val lemma =store_thm("lemma",
     FULL_SIMP_TAC (srw_ss()) [rderives_def] THEN
     SRW_TAC [] [] THEN 
     `0 < SUC m` by DECIDE_TAC THEN
-    `?m1 m2 pfx1 pfx2 sfx1 sfx2 sfx2' nt'.
-           m1 < (SUC m) /\ m2 < (SUC m) /\
+    `∃m1 m2 pfx1 pfx2 sfx1 sfx2 sfx2' nt'.
+           m1 < (SUC m) ∧ m2 < (SUC m) ∧
            NRC (rderives ag) m1 [NTS (startSym ag)]
-             (pfx1 ++ [NTS nt'] ++ sfx1) /\
-           MEM (rule nt' (pfx2 ++ [NTS nt] ++ sfx2)) (rules ag) /\
+             (pfx1 ++ [NTS nt'] ++ sfx1) ∧
+           MEM (rule nt' (pfx2 ++ [NTS nt] ++ sfx2)) (rules ag) ∧
            NRC (rderives ag) m2
              (pfx1 ++ pfx2 ++ [NTS nt] ++ sfx2 ++ sfx1)
-             (pfx1 ++ pfx2 ++ [NTS nt] ++ sfx2' ++ sfx1) /\
-           (pfx = pfx1 ++ pfx2) /\ (sfx = sfx2' ++ sfx1)` 
+             (pfx1 ++ pfx2 ++ [NTS nt] ++ sfx2' ++ sfx1) ∧
+           (pfx = pfx1 ++ pfx2) ∧ (sfx = sfx2' ++ sfx1)` 
 	by METIS_TAC [sublemma] THEN
     SRW_TAC [] [] THEN
-    `?s.(trans ag (initItems ag (rules ag),pfx1) =
-         SOME s) /\ 
+    `∃s.(trans ag (initItems ag (rules ag),pfx1) =
+         SOME s) ∧ 
          MEM (item nt' ([],(pfx2 ++ [NTS nt] ++ sfx2))) s` 
 	by METIS_TAC [] THEN
     METIS_TAC [transShiftExists, initItems]
-    ])
+    ]);
  
 
 
 val transOutEq = store_thm ("transOutEq",
-``!s0 pfx s s'.
-  (trans g (s0,pfx) = SOME s) ==>
-  (trans g (s0,pfx) = SOME s') ==>
+``∀s0 pfx s s'.
+  (trans g (s0,pfx) = SOME s) ⇒
+  (trans g (s0,pfx) = SOME s') ⇒
   (s=s')``,
-Induct_on `pfx` THEN SRW_TAC [] [trans])
+Induct_on `pfx` THEN SRW_TAC [] [trans]);
     
 
 
@@ -1961,92 +1987,108 @@ val doReduce = Define `doReduce m ((sym::rst), os, ((s, itl)::rem)) ru =
 						let 
 						    ns = ((NTS l), nx)
 						in 
-						    SOME ((sym::rst),([(ns,p)] ++ newStk), push newStateStk ns)`
+						    SOME ((sym::rst),([(ns,p)] ++ newStk), push newStateStk ns)`;
 
 
+(*!!!!Make this followSetML*)
 val red_eq1 = store_thm ("red_eq1",
-``~(TS sym IN followSetML g (NTS s)) ==>
+``~(TS sym IN followSet g (NTS s)) ⇒
 (reduce g itl sym = reduce g (item s (q,[])::itl) sym)``,
-SRW_TAC [] [reduce])
 
+SRW_TAC [] [reduce]);
 
+(*!!!!Make this followSetML*)
 val red_eq2 = store_thm ("red_eq2",
-``(TS sym IN followSetML g (NTS s)) ==>
+``(TS sym IN followSet g (NTS s)) ⇒
 ((rule s q::reduce g itl sym) = reduce g (item s (q,[])::itl) sym)``,
-SRW_TAC [] [reduce])
+SRW_TAC [] [reduce]);
 
 
+(*!!!!Make this followSetML*)
 val reduce_mem = store_thm ("reduce_mem", 
-``!sym itl out.(reduce g itl sym = out) ==> 
-(!e.MEM e out ==> ?l r1.(e=rule l r1) /\ (MEM (item l (r1,[])) itl))``,
-Induct_on `itl` THEN SRW_TAC [] [] THENL[
-Cases_on `sym` THEN FULL_SIMP_TAC (srw_ss()) [reduce],
+``∀sym itl out.(reduce g itl sym = out) ⇒ 
+(∀e.MEM e out ⇒ ∃l r1.(e=rule l r1) ∧ (MEM (item l (r1,[])) itl))``,
+
+Induct_on `itl` THEN SRW_TAC [] [] THEN1
+(Cases_on `e` THEN FULL_SIMP_TAC (srw_ss()) [reduce]) THEN
 Cases_on `h` THEN Cases_on `p` THEN
 Cases_on `r` THEN
-FULL_SIMP_TAC (srw_ss() ++ DNF_ss) [doReduce, LET_THM, option_case_rwt, list_case_rwt, pairTheory.FORALL_PROD] THENL[
-Cases_on `(TS sym) IN (followSetML g (NTS s))` THENL[
-`MEM e ((rule s q)::reduce g itl sym)` by METIS_TAC [red_eq2] THEN
-`(e=rule s q) \/ (MEM e (reduce g itl sym))` by METIS_TAC [MEM] THENL[
-Cases_on `e` THEN
-METIS_TAC [reduce, red_eq1],
-METIS_TAC [MEM]],
-METIS_TAC [MEM , reduce]],
-METIS_TAC [MEM , reduce]]])
+FULL_SIMP_TAC (srw_ss() ++ DNF_ss) [doReduce, LET_THM, option_case_rwt, 
+ list_case_rwt, pairTheory.FORALL_PROD] 
+THENL[
+
+ Cases_on `(TS sym) IN (followSet g (NTS n))` THENL[
+ `MEM e ((rule n q)::reduce g itl sym)` by METIS_TAC [red_eq2] THEN
+ `(e=rule n q) ∨ (MEM e (reduce g itl sym))` by METIS_TAC [MEM] THENL[
+ Cases_on `e` THEN
+ METIS_TAC [reduce, red_eq1],
+ METIS_TAC [MEM]],
+ METIS_TAC [MEM , reduce]],
+
+ METIS_TAC [MEM , reduce]]);
+
 
 
 val getstate_red = store_thm ("getstate_red", 
-``!m itl sym g.(m = (sgoto g, reduce g)) ==> 
-validItl g itl ==> (getState m itl sym = REDUCE r) ==> MEM r (rules g)``,
+``∀m itl sym g.(m = (sgoto g, reduce g)) ⇒ isTmnlSym sym ⇒
+validItl g itl ⇒ (getState m itl sym = REDUCE r) ⇒ MEM r (rules g)``,
+
 SRW_TAC [] [] THEN
 FULL_SIMP_TAC (srw_ss()) [getState, LET_THM] THEN
-Cases_on `sgoto g itl sym` THEN Cases_on `reduce g itl (sym2Str sym)` THEN FULL_SIMP_TAC (srw_ss()) [] THENL[
-Cases_on `~(LENGTH t = 0)` THEN FULL_SIMP_TAC (srw_ss()) [] THEN
-Cases_on `sym` THEN Induct_on `itl` THEN
-SRW_TAC [] [] THEN
-FULL_SIMP_TAC (srw_ss()) [reduce] THEN `t=[]` by METIS_TAC [LENGTH_NIL] THEN
-SRW_TAC [] [] THEN
-
-`!e.MEM e [h] ==>
-         ?l r1. (e = rule l r1) /\ MEM (item l (r1,[])) (h'::itl)` by METIS_TAC [reduce_mem] THEN
+Cases_on `sgoto g itl sym` THEN 
+Cases_on `reduce g itl (ts2str sym)` THEN FULL_SIMP_TAC (srw_ss()) [] 
+THENL[
+ Cases_on `~(LENGTH t = 0)` THEN FULL_SIMP_TAC (srw_ss()) [] THEN
+ Cases_on `sym` THEN Induct_on `itl` THEN
+ SRW_TAC [] [] THEN
+ FULL_SIMP_TAC (srw_ss()) [reduce] THEN `t=[]` by METIS_TAC [LENGTH_NIL] THEN
+ SRW_TAC [] [] THEN
+ FULL_SIMP_TAC (srw_ss()) [isTmnlSym_def] THEN
+ `∀e.MEM e [h] ⇒
+ ∃l r1. (e = rule l r1) ∧ MEM (item l (r1,[])) (h'::itl)` by METIS_TAC [reduce_mem] THEN
 FULL_SIMP_TAC (srw_ss()) [reduce_mem,validItl, THE_DEF, APPEND, CONS, EVERY_DEF] THEN
 `validItl g [h']` by METIS_TAC [APPEND, validItl_append] THEN
-METIS_TAC [reduce_mem,validItl, APPEND, CONS, EVERY_DEF, MEM, validItl_append, rgr_r9eq, APPEND_NIL],
+METIS_TAC [reduce_mem,validItl, APPEND, CONS, EVERY_DEF, MEM, validItl_append, rgr_r9eq, 
+ APPEND_NIL],
 
 Cases_on `itemEqRuleList (h::t) (h'::t')` THEN FULL_SIMP_TAC (srw_ss()) [] THEN
-`!e.MEM e (h'::t') ==>
-         ?l r1. (e = rule l r1) /\ MEM (item l (r1,[])) itl` by METIS_TAC [reduce_mem]
+`∀e.MEM e (h'::t') ⇒
+         ∃l r1. (e = rule l r1) ∧ MEM (item l (r1,[])) itl` by METIS_TAC [reduce_mem]
 THEN
 FULL_SIMP_TAC (srw_ss()) [reduce_mem,validItl, THE_DEF, APPEND, CONS, EVERY_DEF] THEN
-METIS_TAC [reduce_mem,validItl, APPEND, CONS, EVERY_DEF, MEM, validItl_append, rgr_r9eq, APPEND_NIL]]
-)
+METIS_TAC [reduce_mem,validItl, APPEND, CONS, EVERY_DEF, MEM, validItl_append, rgr_r9eq, 
+APPEND_NIL]]);
+
 
 val getState_mem_itl = store_thm ("getState_mem_itl", 
-``validItl g itl ==> (m = (sgoto g, reduce g)) ==> 
-(getState m itl e = REDUCE (rule s' l)) ==> (MEM (item s' (l,[])) itl)``,
+``validItl g itl ⇒ (m = (sgoto g, reduce g)) ⇒ isTmnlSym e ⇒
+(getState m itl e = REDUCE (rule s' l)) ⇒ (MEM (item s' (l,[])) itl)``,
+
 SRW_TAC [] [] THEN
 `MEM (rule s' l) (rules g)` by METIS_TAC [getstate_red] THEN
 FULL_SIMP_TAC (srw_ss()) [getState, LET_THM] THEN
-Cases_on `sgoto g itl e` THEN Cases_on `reduce g itl (sym2Str e)` THEN FULL_SIMP_TAC (srw_ss()) []  THENL[
+Cases_on `sgoto g itl e` THEN Cases_on `reduce g itl (ts2str e)` THEN 
+FULL_SIMP_TAC (srw_ss()) [isTmnlSym_def]  THENL[
 Cases_on `LENGTH t = 0` THEN FULL_SIMP_TAC (srw_ss()) [] THEN
 SRW_TAC [] [] THEN
 `MEM (rule s' l) (rule s' l::t)` by METIS_TAC [MEM] THEN
-`?l' r1. (rule s' l = rule l' r1) /\ MEM (item l' (r1,[])) itl` by METIS_TAC [reduce_mem] THEN
+`∃l' r1. (rule s' l = rule l' r1) ∧ MEM (item l' (r1,[])) itl` by METIS_TAC [reduce_mem] THEN
 FULL_SIMP_TAC (srw_ss()) [],
 
 Cases_on `itemEqRuleList (h::t) (h'::t')` THEN FULL_SIMP_TAC (srw_ss()) [] THEN
 SRW_TAC [] [] THEN
 `MEM (rule s' l) (rule s' l::t')` by METIS_TAC [MEM] THEN
-`?l' r1. (rule s' l = rule l' r1) /\ MEM (item l' (r1,[])) itl` by METIS_TAC [reduce_mem] THEN
-FULL_SIMP_TAC (srw_ss()) []]) 
+`∃l' r1. (rule s' l = rule l' r1) ∧ MEM (item l' (r1,[])) itl` by METIS_TAC [reduce_mem] THEN
+FULL_SIMP_TAC (srw_ss()) []]);
 
 
 val validItl_initProds2Items = store_thm ("validItl_initProds2Items", 
-``!g l.validItl g (initProds2Items sym (rules g))``,
+``∀g l.validItl g (initProds2Items sym (rules g))``,
 Cases_on `g` THEN SRW_TAC [] [rules_def] THEN
 Induct_on `l` THEN SRW_TAC [] [initProds2Items, validItl, rules_def] THEN
 Cases_on `h` THEN
 SRW_TAC [] [initProds2Items, validItl, rules_def] THEN
-METIS_TAC [validItl_rules_cons])
+METIS_TAC [validItl_rules_cons]);
 
 
 
@@ -2071,22 +2113,23 @@ val parse = Define `
 		       || (GOTO st) -> 
 			 if (isNonTmnlSym sym) then NONE 
 			 else (* shift goto *) 
-			     SOME (rst,((sym,st),Leaf (sym2Str sym))::os, push ((s, itl)::rem) (sym,st))
-			   || (REDUCE ru) -> doReduce m ((sym::rst), os, ((s, itl)::rem)) ru))`
+			     SOME (rst,((sym,st),Leaf (ts2str sym))::os, push ((s, itl)::rem) (sym,st))
+			   || (REDUCE ru) -> doReduce m ((sym::rst), os, ((s, itl)::rem)) ru))`;
     
 
 
 (* parser :: machine -> symbol list -> ((state,ptree) list -> ptree option *)
-val stackSyms = Define `stackSyms stl = (REVERSE (MAP FST (MAP FST stl)))`
+val stackSyms = Define `stackSyms stl = (REVERSE (MAP FST (MAP FST stl)))`;
 
 val exitCond = Define 
 `exitCond (eof,oldSym)  (inp,stl,csl) =  
-    (~(stl=([]:((symbol # state) # ptree) list)) /\ 
-     (stackSyms stl = [oldSym]) /\ 
-     (inp = [TS eof]))`
+    (~(stl=([]:((('nts,'ts)symbol # ('nts,'ts)state) # ('nts,'ts)ptree) list)) ∧ 
+     (stackSyms stl = [oldSym]) ∧ 
+     (inp = [TS eof]))`;
 
 val init = Define
-`init inis sl =  (sl,([]:((symbol# state) # ptree) list),[inis])`
+`init inis sl =  
+(sl,([]:((('nts,'ts)symbol# ('nts,'ts)state) # ('nts,'ts)ptree) list),[inis])`;
 
 val parser = Define `parser (initState, eof, oldS) m sl = 
 let 
@@ -2096,7 +2139,7 @@ in
     case out of NONE -> NONE
               || (SOME (SOME (slo,[(st1,pt)],cs))) -> SOME (SOME pt)
 	     || SOME (NONE) -> SOME (NONE)
-	|| SOME _ -> SOME NONE`
+	|| SOME _ -> SOME NONE`;
 
 
 
@@ -2118,14 +2161,14 @@ in
 	  case (parser (initState,eof,startSym g) (SOME m) sl) 
 	   of NONE -> NONE
 		|| SOME (NONE) -> NONE
-		|| SOME (SOME out) -> SOME out))`
+		|| SOME (SOME out) -> SOME out))`;
 
 
 
 val parseExp = store_thm
 ("parseExp",
-``!Q.(\(x,y,z).parse Q (x,y,z)) = parse Q``,
-SRW_TAC [] [FUN_EQ_THM,UNCURRY])
+``∀Q.(\(x,y,z).parse Q (x,y,z)) = parse Q``,
+SRW_TAC [] [FUN_EQ_THM,UNCURRY]);
 
 
 val mlDir = ref ("./theoryML/");
@@ -2135,7 +2178,7 @@ val list_size_def =
   REWRITE_RULE [arithmeticTheory.ADD_ASSOC]
                (#2 (TypeBase.size_of ``:'a list``));*)
 
-
+(*
 val _ =
  let open EmitML
  in emitML (!mlDir)
@@ -2172,16 +2215,16 @@ val _ =
     :: [])
  end;
 
-
+*)
 (*
 Theorems
-1. ?g.~(yacc g = NONE)
+1. ∃g.~(yacc g = NONE)
 
-2. s IN language (g) /\ (yacc (g) = SOME lrm) ==> ?t.(parse lrm s = SOME (t))
+2. s IN language (g) ∧ (yacc (g) = SOME lrm) ⇒ ∃t.(parse lrm s = SOME (t))
 
-3. (yacc g = SOME lrm) ==> unambiguous (g)
+3. (yacc g = SOME lrm) ⇒ unambiguous (g)
 
-4. (yacc g sl = SOME tree) ==> (validptree tree g /\ (leaves tree = sl))
+4. (yacc g sl = SOME tree) ⇒ (validptree tree g ∧ (leaves tree = sl))
 
 *)
 
